VHDL_Hoare_Complete.thy
@@ -14,12 +14,12 @@ begin
 
 subsection "A sound and complete Hoare logic for VHDL's sequential statements"
 
-text \<open>This theory is the second attempt for defining a Hoare logic for VHDL's sequential statement. 
-As shown in the very last part of this theory, we prove that this definition is both sound and 
+text \<open>This theory is the second attempt for defining a Hoare logic for VHDL's sequential statement.
+As shown in the very last part of this theory, we prove that this definition is both sound and
 complete.\<close>
 
-typedef (overloaded) ('signal) worldline2 = 
-  "{w :: 'signal worldline . (\<exists>t. \<forall>t'. t' > t \<longrightarrow> (\<lambda>s. w s t') = (\<lambda>s. w s t))}" 
+typedef (overloaded) ('signal) worldline2 =
+  "{w :: 'signal worldline . (\<exists>t. \<forall>t'. t' > t \<longrightarrow> (\<lambda>s. w s t') = (\<lambda>s. w s t))}"
   morphisms Rep_worldline Abs_worldline
 proof -
   define wit :: "'signal worldline" where "wit \<equiv> (\<lambda>s t. False)"
@@ -31,8 +31,8 @@ qed
 
 setup_lifting type_definition_worldline2
 
-text \<open> The reason why the first attempt of defining the semantics in @{theory Draft.VHDL_Hoare} is 
-not complete is because not all worldline can be transformed into elements of the operational 
+text \<open> The reason why the first attempt of defining the semantics in @{theory Draft.VHDL_Hoare} is
+not complete is because not all worldline can be transformed into elements of the operational
 semantics, especially the transaction @{term "\<tau> :: 'signal transaction"}. Why is this so?
 
 Imagine a worldline @{term "w"} where it always alternate between @{term "True :: val"} and @{term
@@ -42,7 +42,7 @@ because it will have infinite mappings (since it constantly changes the value be
 :: val"} and @{term "False :: val"}, and a @{typ "'signal transaction"} needs to be zero at nearly
 everywhere, i.e., eventually the mapping will ``die out''.
 
-The typedef of @{typ "'signal worldline2"} imposes that eventually there will be no more mapping. 
+The typedef of @{typ "'signal worldline2"} imposes that eventually there will be no more mapping.
 Hence, when we attempt to find its derivative, we can construct a @{typ "'signal transaction"}.
 \<close>
 
@@ -51,7 +51,7 @@ definition worldline_deg :: "'signal worldline2 \<Rightarrow> nat" where
 
 lemma existence_of_degree:
   fixes w :: "'signal worldline2"
-  shows "\<exists>x. \<forall>t > x. \<forall>s. Rep_worldline w s t = Rep_worldline w s x" 
+  shows "\<exists>x. \<forall>t > x. \<forall>s. Rep_worldline w s t = Rep_worldline w s x"
   by transfer meson
 
 lemma property_of_degree:
@@ -60,11 +60,11 @@ lemma property_of_degree:
   shows "\<forall>t > d. \<forall>s. Rep_worldline w s t = Rep_worldline w s d"
   using LeastI_ex[OF existence_of_degree] unfolding d_def worldline_deg_def by auto
 
-lift_definition worldline_upd2 :: 
+lift_definition worldline_upd2 ::
   "'signal worldline2 \<Rightarrow> 'signal \<Rightarrow> nat \<Rightarrow> val \<Rightarrow> 'signal worldline2" ("_[_, _:=\<^sub>2 _]")
   is worldline_upd
 proof -
-  fix w :: "'signal \<Rightarrow> nat \<Rightarrow> val" 
+  fix w :: "'signal \<Rightarrow> nat \<Rightarrow> val"
   fix sig v
   fix t :: nat
   assume "\<exists>t. \<forall>t'>t. (\<lambda>s'. w s' t') = (\<lambda>s'. w s' t)"
@@ -87,25 +87,25 @@ proof -
   ultimately show "\<exists>t''. \<forall>t'>t''. (\<lambda>s. w[sig, t:= v] s t') = (\<lambda>s. w[sig, t:= v] s t'')"
     by auto
 qed
-        
-lift_definition worldline_inert_upd2 :: 
+
+lift_definition worldline_inert_upd2 ::
   "'signal worldline2 \<Rightarrow> 'signal \<Rightarrow> nat \<Rightarrow> nat \<Rightarrow> val \<Rightarrow> 'signal worldline2" ("_[_, _, _ :=\<^sub>2 _]")
-  is worldline_inert_upd 
+  is worldline_inert_upd
 proof -
-  fix w :: "'signal \<Rightarrow> nat \<Rightarrow> val" 
+  fix w :: "'signal \<Rightarrow> nat \<Rightarrow> val"
   fix sig v
-  fix t1 t2 :: nat  
+  fix t1 t2 :: nat
   assume "\<exists>t. \<forall>t'>t. (\<lambda>s'. w s' t') = (\<lambda>s'. w s' t)"
   then obtain tcurr :: "nat" where *: "\<forall>t' > tcurr. (\<lambda>s'. w s' t') = (\<lambda>s'. w s' tcurr)"
     by auto
   have "t1 + t2 < tcurr \<or> tcurr \<le> t1 + t2"
-    by auto  
+    by auto
   moreover
   { assume "t1 + t2 < tcurr"
     hence "\<forall>t'> tcurr. (\<lambda>s. w[sig, t1, t2 := v] s t') = (\<lambda>s. w[sig, t1, t2 := v] s tcurr)"
       by (metis "*" le_add1 le_less_trans less_irrefl_nat order.strict_trans  worldline_inert_upd_def)
     hence "\<exists>t''. \<forall>t'> t''. (\<lambda>s. w[sig, t1, t2:= v] s t') = (\<lambda>s. w[sig, t1, t2:= v] s t'')"
-      by auto }    
+      by auto }
   moreover
   { assume "tcurr \<le> t1 + t2"
     have "\<forall>t'> t1 + t2. (\<lambda>s. w[sig, t1, t2 := v] s t') = (\<lambda>s. w[sig, t1, t2 := v] s (t1 + t2))"
@@ -128,9 +128,9 @@ proof -
         by auto
     qed
     hence "\<exists>t''. \<forall>t'> t''. (\<lambda>s. w[sig, t1, t2:= v] s t') = (\<lambda>s. w[sig, t1, t2:= v] s t'')"
-      by auto }   
+      by auto }
   ultimately show "\<exists>t''. \<forall>t'> t''. (\<lambda>s. w[sig, t1, t2:= v] s t') = (\<lambda>s. w[sig, t1, t2:= v] s t'')"
-    by auto 
+    by auto
 qed
 
 lift_definition state_of_world2 :: "'signal worldline2 \<Rightarrow> nat \<Rightarrow> 'signal state" is
@@ -139,14 +139,14 @@ lift_definition state_of_world2 :: "'signal worldline2 \<Rightarrow> nat \<Right
 lift_definition event_of_world2 :: "'signal worldline2 \<Rightarrow> nat \<Rightarrow> 'signal event" is
   event_of_world .
 
-lift_definition beh_of_world2 :: "'signal worldline2 \<Rightarrow> nat \<Rightarrow> 'signal transaction" is 
+lift_definition beh_of_world2 :: "'signal worldline2 \<Rightarrow> nat \<Rightarrow> 'signal transaction" is
   beh_of_world_raw  unfolding beh_of_world_raw_def zero_map by auto
 
 lemma [simp]:
   "beh_of_world2 w 0 = 0"
   by (transfer', auto simp add:  beh_of_world_raw_def zero_option_def zero_fun_def)
 
-lift_definition beval_world2 :: "'signal worldline2 \<Rightarrow> nat \<Rightarrow> 'signal bexp \<Rightarrow> val" 
+lift_definition beval_world2 :: "'signal worldline2 \<Rightarrow> nat \<Rightarrow> 'signal bexp \<Rightarrow> val"
   is beval_world .
 
 type_synonym 'signal assn2 = "'signal worldline2 \<Rightarrow> bool"
@@ -220,8 +220,8 @@ lemma Assign'_hoare2:
 
 subsection \<open>Validity of Hoare proof rules\<close>
 
-lift_definition worldline2 :: 
-  "nat \<Rightarrow> 'signal state \<Rightarrow> 'signal transaction \<Rightarrow> 'signal transaction \<Rightarrow> 'signal worldline2" 
+lift_definition worldline2 ::
+  "nat \<Rightarrow> 'signal state \<Rightarrow> 'signal transaction \<Rightarrow> 'signal transaction \<Rightarrow> 'signal worldline2"
   is worldline
 proof -
   fix t0 :: nat
@@ -236,7 +236,7 @@ proof -
     assume "max last t0 < t'"
     { fix s
       have *: "\<And>n. max last t0 < n \<Longrightarrow> n \<le> t' \<Longrightarrow> lookup \<tau> n = 0"
-        by (simp add: beyond_degree_lookup_zero local.last_def)          
+        by (simp add: beyond_degree_lookup_zero local.last_def)
       have "worldline t0 \<sigma> \<theta> \<tau> s t' = signal_of2 (\<sigma> s) \<tau> s t'"
         by (meson \<open>max last t0 < t'\<close> less_imp_not_less less_max_iff_disj worldline_def)
       also have "... = signal_of2 (\<sigma> s) \<tau> s (max last t0)"
@@ -264,13 +264,13 @@ proof -
     have "\<forall>n > d. Rep_worldline w s n = Rep_worldline w s d"
       using property_of_degree unfolding d_def by auto
     hence "\<forall>n > d. Rep_worldline w s n = Rep_worldline w s (n - 1)"
-      by (metis (full_types) diff_Suc_1 gr0_implies_Suc less_add_same_cancel2 less_imp_Suc_add 
+      by (metis (full_types) diff_Suc_1 gr0_implies_Suc less_add_same_cancel2 less_imp_Suc_add
       less_linear not_add_less1 trans_less_add1) }
   thus ?thesis
     unfolding difference_def unfolding zero_fun_def by (simp add: zero_option_def)
 qed
 
-lift_definition derivative :: "'signal worldline2 \<Rightarrow> nat \<Rightarrow> 'signal transaction" 
+lift_definition derivative :: "'signal worldline2 \<Rightarrow> nat \<Rightarrow> 'signal transaction"
   is "\<lambda>w t n. if n < t then Map.empty else if n = t then Some o (\<lambda>s. Rep_worldline w s t) else difference w n"
   unfolding sym[OF eventually_cofinite] MOST_nat
 proof -
@@ -285,14 +285,24 @@ proof -
     by blast
 qed
 
-definition destruct_worldline :: 
-  "'signal worldline2 \<Rightarrow> nat \<Rightarrow> ('signal state \<times> 'signal event \<times> 'signal transaction \<times> 'signal transaction)" 
+definition destruct_worldline ::
+  "'signal worldline2 \<Rightarrow> nat \<Rightarrow> ('signal state \<times> 'signal event \<times> 'signal transaction \<times> 'signal transaction)"
   where
-  "destruct_worldline w t = (let \<sigma> = (\<lambda>s. Rep_worldline w s t); 
+  "destruct_worldline w t = (let \<sigma> = (\<lambda>s. Rep_worldline w s t);
                                  \<theta> = poly_mapping_of_fun (\<lambda>t. Some o (\<lambda>s. (Rep_worldline w) s t)) 0 t;
-                                 \<gamma> = {s. \<sigma> s \<noteq> signal_of2 False \<theta> s (t - 1)}; 
-                                 \<tau> = derivative_raw (Rep_worldline w) (worldline_deg w) t 
+                                 \<gamma> = {s. \<sigma> s \<noteq> signal_of2 False \<theta> s (t - 1)};
+                                 \<tau> = derivative_raw (Rep_worldline w) (worldline_deg w) t
                              in (\<sigma>, \<gamma>, \<theta>, \<tau>))"
+
+text \<open>One might concern about the event @{term "\<gamma> :: 'signal event"} obtained from the destruction
+@{term "destruct_worldline w t"} above. What happens if @{term "t = 0"}? This is a valid concern
+since we have the expression @{term "t - 1"} in the definition of @{term "\<gamma>"} above.
+
+Note that, we impose the requirement of @{term "context_invariant"} here. When this is the case,
+history @{term "\<theta> :: 'signal transaction"} is empty when @{term "t = 0"}. Hence the expression
+@{term "signal_of2 False \<theta> s (t - 1)"} is equal to @{term "signal_of2 False empty_trans s 0"} and,
+subsequently, equals to @{term "False"}. Hence, when @{term "t = 0"}, the @{term "\<gamma>"} enumerates the
+signals which are different with the default value @{term "False :: val"}.\<close>
 
 lemma destruct_worldline_exist:
   "\<exists>\<sigma> \<gamma> \<theta> \<tau>. destruct_worldline w t = (\<sigma>, \<gamma>, \<theta>, \<tau>)"
@@ -308,33 +318,33 @@ proof -
   thus ?thesis
     using assms unfolding destruct_worldline_def Let_def worldline_deg_def
   proof transfer'
-    fix w :: "'signal worldline" 
-    fix t \<sigma> \<gamma> 
+    fix w :: "'signal worldline"
+    fix t \<sigma> \<gamma>
     fix \<theta> \<tau> :: "'signal transaction"
     assume *: "\<exists>t. \<forall>t'>t. (\<lambda>s. w s t') = (\<lambda>s. w s t)"
     then obtain d where d_def: "d = (LEAST t. \<forall>t'>t. (\<lambda>s. w s t') = (\<lambda>s. w s t))"
       by auto
-    have d_prop: "\<forall>t'>d. (\<lambda>s. w s t') = (\<lambda>s. w s d)" 
-      using LeastI_ex[OF *] unfolding d_def  by blast 
+    have d_prop: "\<forall>t'>d. (\<lambda>s. w s t') = (\<lambda>s. w s d)"
+      using LeastI_ex[OF *] unfolding d_def  by blast
     hence d_prop': "\<And>n s. d < n \<Longrightarrow> w s n = w s d"
       by meson
     have d_def': "d = (LEAST n. \<forall>t>n. \<forall>s. w s t = w s n)"
       unfolding d_def  by metis
     assume **:
-      "(\<lambda>s. w s t, 
-        {s. w s t \<noteq> signal_of2 False (poly_mapping_of_fun (\<lambda>t. Some \<circ> (\<lambda>s. w s t)) 0 t) s (t - 1)}, 
+      "(\<lambda>s. w s t,
+        {s. w s t \<noteq> signal_of2 False (poly_mapping_of_fun (\<lambda>t. Some \<circ> (\<lambda>s. w s t)) 0 t) s (t - 1)},
         poly_mapping_of_fun (\<lambda>t. Some \<circ> (\<lambda>s. w s t)) 0 t,
-        derivative_raw w (LEAST n. \<forall>t>n. \<forall>s. w s t = w s n) t) = (\<sigma>, \<gamma>, \<theta>, \<tau>)"  
-    hence \<sigma>_def: "\<sigma> = (\<lambda>s. w s t)" and 
+        derivative_raw w (LEAST n. \<forall>t>n. \<forall>s. w s t = w s n) t) = (\<sigma>, \<gamma>, \<theta>, \<tau>)"
+    hence \<sigma>_def: "\<sigma> = (\<lambda>s. w s t)" and
           \<gamma>_def: "\<gamma> = {s. w s t \<noteq> signal_of2 False (poly_mapping_of_fun (\<lambda>t. Some \<circ> (\<lambda>s. w s t)) 0 t) s (t - 1)}" and
           \<theta>_def: "\<theta> = poly_mapping_of_fun (\<lambda>t. Some \<circ> (\<lambda>s. w s t)) 0 t"
       by auto
     have \<tau>_def: "\<tau> = derivative_raw w d t"
-      using ** unfolding d_def' by auto 
+      using ** unfolding d_def' by auto
     have "w = worldline t \<sigma> \<theta> \<tau>"
     proof (rule ext, rule ext, cases "t \<le> d")
       case True
-      fix s' t' 
+      fix s' t'
       have "t' < t \<or> t \<le> t'" by auto
       moreover
       { assume "t' < t"
@@ -356,7 +366,7 @@ proof -
         by auto
     next
       case False
-      fix s' t' 
+      fix s' t'
       have "t' < t \<or> t \<le> t'" by auto
       moreover
       { assume "t' < t"
@@ -386,7 +396,7 @@ proof -
     have "\<forall>n. t \<le> n \<longrightarrow> lookup \<theta> n = 0"
       unfolding \<theta>_def apply transfer' by auto
     moreover have "\<forall>n. n < t \<longrightarrow> lookup \<tau> n = 0"
-      unfolding \<tau>_def 
+      unfolding \<tau>_def
       by (transfer', metis (mono_tags) derivative_raw.rep_eq derivative_raw_zero lookup_zero)
     moreover have "\<forall>s. s \<in> dom (lookup \<tau> t) \<longrightarrow> \<sigma> s = the (lookup \<tau> t s)"
       unfolding \<tau>_def \<sigma>_def by transfer' auto
@@ -399,7 +409,7 @@ qed
 
 lemma worldline2_constructible':
   fixes w :: "'signal worldline2"
-  fixes t :: nat                                     
+  fixes t :: nat
   shows "\<exists>\<sigma> \<gamma> \<theta> \<tau>. w = worldline2 t \<sigma> \<theta> \<tau> \<and> context_invariant t \<sigma> \<gamma> \<theta> \<tau>"
   by (meson destruct_worldline_def worldline2_constructible)
 
@@ -409,7 +419,7 @@ lemma state_worldline2:
   using assms
 proof (intro ext, transfer')
   fix s t \<sigma>
-  fix \<gamma> :: "'a event" 
+  fix \<gamma> :: "'a event"
   fix \<theta> \<tau>
   assume ci: "context_invariant t \<sigma> \<gamma> \<theta> \<tau>"
   hence "\<And>n. n < t \<Longrightarrow> lookup \<tau> n = 0"
@@ -417,7 +427,7 @@ proof (intro ext, transfer')
   have "lookup \<tau> t s = 0 \<or> lookup \<tau> t s \<noteq> 0" by auto
   moreover
   { assume "lookup \<tau> t s \<noteq> 0"
-    hence "s \<in> dom (lookup \<tau> t)"      
+    hence "s \<in> dom (lookup \<tau> t)"
       by (metis domIff zero_fun_def zero_map)
     hence "\<sigma> s = the (lookup \<tau> t s)"
       using ci unfolding context_invariant_def by auto
@@ -438,7 +448,7 @@ proof (intro ext, transfer')
         using `\<And>n. n < t \<Longrightarrow> lookup \<tau> n = 0` `lookup \<tau> t s = 0` `k \<le> t`
         by (metis antisym_conv1 zero_fun_def)
       moreover have "lookup \<tau> k s \<noteq> 0"
-        using k_dom unfolding domIff zero_option_def apply transfer' unfolding to_trans_raw2_def 
+        using k_dom unfolding domIff zero_option_def apply transfer' unfolding to_trans_raw2_def
         by auto
       ultimately show "False"
         by auto
@@ -446,7 +456,7 @@ proof (intro ext, transfer')
     hence "inf_time (to_transaction2 \<tau>) s t = None"
       by (intro inf_time_noneI)
     hence "signal_of2 (\<sigma> s) \<tau> s t = \<sigma> s"
-      unfolding to_signal2_def comp_def by auto 
+      unfolding to_signal2_def comp_def by auto
     hence "worldline t \<sigma> \<theta> \<tau> s t = \<sigma> s"
       unfolding worldline_def by auto }
   ultimately show "worldline t \<sigma> \<theta> \<tau> s t = \<sigma> s"
@@ -455,12 +465,12 @@ qed
 
 lemma history_worldline2:
   assumes "context_invariant t \<sigma> \<gamma> \<theta> \<tau>"
-  shows "signal_of2 False (poly_mapping_of_fun (\<lambda>ta. Some \<circ> (\<lambda>s. Rep_worldline (worldline2 t \<sigma> \<theta> \<tau>) s ta)) 0 t) s (t - 1) = 
+  shows "signal_of2 False (poly_mapping_of_fun (\<lambda>ta. Some \<circ> (\<lambda>s. Rep_worldline (worldline2 t \<sigma> \<theta> \<tau>) s ta)) 0 t) s (t - 1) =
          signal_of2 False \<theta> s (t - 1)"
   using assms
 proof transfer'
-  fix t \<sigma> 
-  fix \<gamma> :: "'a event" 
+  fix t \<sigma>
+  fix \<gamma> :: "'a event"
   fix \<theta> \<tau> s
   assume "context_invariant t \<sigma> \<gamma> \<theta> \<tau>"
   hence "lookup \<theta> t = 0"
@@ -474,7 +484,7 @@ proof transfer'
          lookup (poly_mapping_of_fun (\<lambda>taa. Some \<circ> (\<lambda>s. worldline t \<sigma> \<theta> \<tau> s taa)) 0 t) n =
          lookup (poly_mapping_of_fun (\<lambda>taa. Some \<circ> (\<lambda>s. signal_of2 False \<theta> s taa)) 0 t) n"
       apply transfer' unfolding worldline_def by auto
-    have " signal_of2 False (poly_mapping_of_fun (\<lambda>ta. Some \<circ> (\<lambda>s. worldline t \<sigma> \<theta> \<tau> s ta)) 0 t) s (t - 1) = 
+    have " signal_of2 False (poly_mapping_of_fun (\<lambda>ta. Some \<circ> (\<lambda>s. worldline t \<sigma> \<theta> \<tau> s ta)) 0 t) s (t - 1) =
            signal_of2 False (poly_mapping_of_fun (\<lambda>taa. Some \<circ> (\<lambda>s. signal_of2 False \<theta> s taa)) 0 t) s (t - 1)"
       using signal_of2_lookup_same[OF *] by auto
     also have "... = signal_of2 False \<theta> s (t - 1)"
@@ -483,46 +493,46 @@ proof transfer'
       by auto }
   moreover
   { assume "t = 0"
-    hence "signal_of2 False (poly_mapping_of_fun (\<lambda>ta. Some \<circ> (\<lambda>s. worldline t \<sigma> \<theta> \<tau> s ta)) 0 t) s (t - 1) = 
+    hence "signal_of2 False (poly_mapping_of_fun (\<lambda>ta. Some \<circ> (\<lambda>s. worldline t \<sigma> \<theta> \<tau> s ta)) 0 t) s (t - 1) =
            signal_of2 False (poly_mapping_of_fun (\<lambda>ta. Some \<circ> (\<lambda>s. worldline 0 \<sigma> \<theta> \<tau> s ta)) 0 0) s 0"
       by auto
     also have "... =  signal_of2 False 0 s 0"
       unfolding poly_mapping_of_fun_empty_set  by auto
     also have "... = signal_of2 False \<theta> s 0"
-      using `lookup \<theta> t = 0` unfolding `t = 0` using signal_of2_zero 
+      using `lookup \<theta> t = 0` unfolding `t = 0` using signal_of2_zero
       by (metis signal_of2_empty zero_fun_def)
     also have "... = signal_of2 False \<theta> s (t - 1)"
       using `t = 0` by auto
     finally have "signal_of2 False (poly_mapping_of_fun (\<lambda>ta. Some \<circ> (\<lambda>s. worldline t \<sigma> \<theta> \<tau> s ta)) 0 t) s (t - 1) = signal_of2 False \<theta> s (t - 1)"
       by auto }
   ultimately show "signal_of2 False (poly_mapping_of_fun (\<lambda>ta. Some \<circ> (\<lambda>s. worldline t \<sigma> \<theta> \<tau> s ta)) 0 t) s (t - 1) = signal_of2 False \<theta> s (t - 1)"
-    by auto 
+    by auto
 qed
 
 lemma beh_of_worldline:
   assumes "context_invariant t \<sigma> \<gamma> \<theta> \<tau>"
-  shows "\<And>k. signal_of2 False (poly_mapping_of_fun (\<lambda>ta. Some \<circ> (\<lambda>s. Rep_worldline (worldline2 t \<sigma> \<theta> \<tau>) s ta)) 0 t) s k = 
+  shows "\<And>k. signal_of2 False (poly_mapping_of_fun (\<lambda>ta. Some \<circ> (\<lambda>s. Rep_worldline (worldline2 t \<sigma> \<theta> \<tau>) s ta)) 0 t) s k =
              signal_of2 False \<theta> s k"
   using assms
 proof transfer'
-  fix k t \<sigma> 
-  fix \<gamma> :: "'a event" 
-  fix \<theta> \<tau> s 
+  fix k t \<sigma>
+  fix \<gamma> :: "'a event"
+  fix \<theta> \<tau> s
   assume "context_invariant t \<sigma> \<gamma> \<theta> \<tau>"
   hence "lookup \<theta> t = 0"
     unfolding context_invariant_def by auto
-  have *: "\<And>n.       
+  have *: "\<And>n.
        lookup (poly_mapping_of_fun (\<lambda>taa. Some \<circ> (\<lambda>s. worldline t \<sigma> \<theta> \<tau> s taa)) 0 t) n =
        lookup (poly_mapping_of_fun (\<lambda>taa. Some \<circ> (\<lambda>s. signal_of2 False \<theta> s taa)) 0 t) n"
     apply transfer' unfolding worldline_def by auto
-  have **: " signal_of2 False (poly_mapping_of_fun (\<lambda>ta. Some \<circ> (\<lambda>s. worldline t \<sigma> \<theta> \<tau> s ta)) 0 t) s k = 
+  have **: " signal_of2 False (poly_mapping_of_fun (\<lambda>ta. Some \<circ> (\<lambda>s. worldline t \<sigma> \<theta> \<tau> s ta)) 0 t) s k =
          signal_of2 False (poly_mapping_of_fun (\<lambda>taa. Some \<circ> (\<lambda>s. signal_of2 False \<theta> s taa)) 0 t) s k"
     using signal_of2_lookup_same[OF *] by auto
   have "k < t \<or> t \<le> k"
     by auto
-  moreover 
+  moreover
   { assume "k < t"
-    have "signal_of2 False (poly_mapping_of_fun (\<lambda>taa. Some \<circ> (\<lambda>s. signal_of2 False \<theta> s taa)) 0 t) s k 
+    have "signal_of2 False (poly_mapping_of_fun (\<lambda>taa. Some \<circ> (\<lambda>s. signal_of2 False \<theta> s taa)) 0 t) s k
           = signal_of2 False \<theta> s (k)"
       using signal_of2_poly_mapping_fun[OF `k < t`] by metis
     hence "signal_of2 False (poly_mapping_of_fun (\<lambda>ta. Some \<circ> (\<lambda>s. worldline t \<sigma> \<theta> \<tau> s ta)) 0 t) s k = signal_of2 False \<theta> s k"
@@ -540,7 +550,7 @@ proof transfer'
       have "\<And>n. t - 1 < n \<Longrightarrow> n \<le> k \<Longrightarrow> lookup (poly_mapping_of_fun (\<lambda>taa. Some \<circ> (\<lambda>s. signal_of2 False \<theta> s taa)) 0 t) n = 0"
         apply transfer' by auto
       with signal_of2_less_ind[OF this]
-      have "signal_of2 False (poly_mapping_of_fun (\<lambda>taa. Some \<circ> (\<lambda>s. signal_of2 False \<theta> s taa)) 0 t) s k = 
+      have "signal_of2 False (poly_mapping_of_fun (\<lambda>taa. Some \<circ> (\<lambda>s. signal_of2 False \<theta> s taa)) 0 t) s k =
              signal_of2 False (poly_mapping_of_fun (\<lambda>taa. Some \<circ> (\<lambda>s. signal_of2 False \<theta> s taa)) 0 t) s (t - 1)"
         using `t - 1 < k` by auto
       also have "... = signal_of2 False \<theta> s (t - 1)"
@@ -551,7 +561,7 @@ proof transfer'
         using ** by auto }
     moreover
     { assume "t = 0"
-      hence "signal_of2 False (poly_mapping_of_fun (\<lambda>taa. Some \<circ> (\<lambda>s. signal_of2 False \<theta> s taa)) 0 t) s k = 
+      hence "signal_of2 False (poly_mapping_of_fun (\<lambda>taa. Some \<circ> (\<lambda>s. signal_of2 False \<theta> s taa)) 0 t) s k =
             signal_of2 False (poly_mapping_of_fun (\<lambda>taa. Some \<circ> (\<lambda>s. signal_of2 False \<theta> s taa)) 0 0) s k"
         by auto
       also have "... = signal_of2 False 0 s k"
@@ -581,18 +591,18 @@ lemma event_worldline2:
   shows "{s. Rep_worldline (worldline2 t \<sigma> \<theta> \<tau>) s t \<noteq> signal_of2 False (poly_mapping_of_fun (\<lambda>ta. Some \<circ> (\<lambda>s. Rep_worldline (worldline2 t \<sigma> \<theta> \<tau>) s ta)) 0 t) s (t - 1)} = \<gamma>"
   using assms state_worldline2[OF assms]
 proof transfer'
-  fix t \<sigma> 
-  fix \<gamma> :: "'a event" 
+  fix t \<sigma>
+  fix \<gamma> :: "'a event"
   fix \<theta> \<tau>
   assume "context_invariant t \<sigma> \<gamma> \<theta> \<tau>"
   assume *: "(\<lambda>s. worldline t \<sigma> \<theta> \<tau> s t) = \<sigma>"
-  have **: "\<gamma> = {s. \<sigma> s \<noteq> signal_of2 False \<theta> s (t - 1)}"  
+  have **: "\<gamma> = {s. \<sigma> s \<noteq> signal_of2 False \<theta> s (t - 1)}"
     using `context_invariant t \<sigma> \<gamma> \<theta> \<tau>` unfolding context_invariant_def by auto
-  have "{s. worldline t \<sigma> \<theta> \<tau> s t \<noteq> signal_of2 False (poly_mapping_of_fun (\<lambda>ta. Some \<circ> (\<lambda>s. worldline t \<sigma> \<theta> \<tau> s ta)) 0 t) s (t - 1)} = 
+  have "{s. worldline t \<sigma> \<theta> \<tau> s t \<noteq> signal_of2 False (poly_mapping_of_fun (\<lambda>ta. Some \<circ> (\<lambda>s. worldline t \<sigma> \<theta> \<tau> s ta)) 0 t) s (t - 1)} =
         {s. \<sigma> s \<noteq> signal_of2 False (poly_mapping_of_fun (\<lambda>ta. Some \<circ> (\<lambda>s. worldline t \<sigma> \<theta> \<tau> s ta)) 0 t) s (t - 1)}"
     using * by metis
-  moreover have "\<And>s. signal_of2 False \<theta> s (t - 1) = 
-            signal_of2 False (poly_mapping_of_fun (\<lambda>ta. Some \<circ> (\<lambda>s. worldline t \<sigma> \<theta> \<tau> s ta)) 0 t) s (t - 1)" 
+  moreover have "\<And>s. signal_of2 False \<theta> s (t - 1) =
+            signal_of2 False (poly_mapping_of_fun (\<lambda>ta. Some \<circ> (\<lambda>s. worldline t \<sigma> \<theta> \<tau> s ta)) 0 t) s (t - 1)"
     using history_worldline2 by (metis \<open>context_invariant t \<sigma> \<gamma> \<theta> \<tau>\<close> worldline2.rep_eq)
   ultimately have "{s. worldline t \<sigma> \<theta> \<tau> s t \<noteq> signal_of2 False (poly_mapping_of_fun (\<lambda>ta. Some \<circ> (\<lambda>s. worldline t \<sigma> \<theta> \<tau> s ta)) 0 t) s (t - 1)} =
                    {s. \<sigma> s \<noteq> signal_of2 False \<theta> s (t - 1)}"
@@ -603,7 +613,7 @@ qed
 
 lemma transaction_worldline2:
   assumes "context_invariant t \<sigma> \<gamma> \<theta> \<tau>"
-  shows "\<And>k s . signal_of2 (\<sigma> s) (derivative_raw (Rep_worldline (worldline2 t \<sigma> \<theta> \<tau>)) (worldline_deg (worldline2 t \<sigma> \<theta> \<tau>)) t) s k = 
+  shows "\<And>k s . signal_of2 (\<sigma> s) (derivative_raw (Rep_worldline (worldline2 t \<sigma> \<theta> \<tau>)) (worldline_deg (worldline2 t \<sigma> \<theta> \<tau>)) t) s k =
                 signal_of2 (\<sigma> s) \<tau> s k"
   using assms unfolding worldline_deg_def
 proof transfer'
@@ -620,7 +630,7 @@ proof transfer'
   moreover
   { assume "k < t"
     have "signal_of2 (\<sigma> s) (derivative_raw (worldline t \<sigma> \<theta> \<tau>) deg t) s k = \<sigma> s"
-      using signal_of2_derivative_before_now \<open>k < t\<close> by fastforce  
+      using signal_of2_derivative_before_now \<open>k < t\<close> by fastforce
     moreover have "signal_of2 (\<sigma> s) \<tau> s k = \<sigma> s"
     proof -
       have "\<forall>n\<in>dom (lookup (to_transaction2 \<tau> s)). k < n"
@@ -640,8 +650,8 @@ proof transfer'
       thus ?thesis
         unfolding to_signal2_def comp_def by auto
     qed
-    ultimately have "signal_of2 (\<sigma> s) (derivative_raw (worldline t \<sigma> \<theta> \<tau>) deg t) s k = 
-                     signal_of2 (\<sigma> s) \<tau> s k" 
+    ultimately have "signal_of2 (\<sigma> s) (derivative_raw (worldline t \<sigma> \<theta> \<tau>) deg t) s k =
+                     signal_of2 (\<sigma> s) \<tau> s k"
       by auto }
   moreover
   { assume "t \<le> k \<and> k \<le> deg"
@@ -649,7 +659,7 @@ proof transfer'
       using signal_of2_derivative_raw by metis
     also have "... = signal_of2 (\<sigma> s) \<tau> s k"
       unfolding worldline_def using `t \<le> k \<and> k \<le> deg` by auto
-    finally have "signal_of2 (\<sigma> s) (derivative_raw (worldline t \<sigma> \<theta> \<tau>) deg t) s k = 
+    finally have "signal_of2 (\<sigma> s) (derivative_raw (worldline t \<sigma> \<theta> \<tau>) deg t) s k =
                      signal_of2 (\<sigma> s) \<tau> s k"
       by auto }
   moreover
@@ -663,7 +673,7 @@ proof transfer'
         unfolding worldline_def using `t \<le> deg` by auto
       also have "... = signal_of2 (\<sigma> s) \<tau> s k"
         using deg_prop `deg < k` `t \<le> deg` unfolding worldline_def by auto
-      finally have "signal_of2 (\<sigma> s) (derivative_raw (worldline t \<sigma> \<theta> \<tau>) deg t) s k = 
+      finally have "signal_of2 (\<sigma> s) (derivative_raw (worldline t \<sigma> \<theta> \<tau>) deg t) s k =
                     signal_of2 (\<sigma> s) \<tau> s k"
         by auto }
     moreover
@@ -703,47 +713,47 @@ proof transfer'
           have "worldline t \<sigma> \<theta> \<tau> s t = signal_of2 (\<sigma> s) \<tau> s t"
             unfolding worldline_def by auto
           also have "... = \<sigma> s"
-            using `context_invariant t \<sigma> \<gamma> \<theta> \<tau>` 
+            using `context_invariant t \<sigma> \<gamma> \<theta> \<tau>`
             by (metis calculation state_worldline2 worldline2.rep_eq)
           finally have "worldline t \<sigma> \<theta> \<tau> s t = \<sigma> s"
             by auto
           hence ?thesis
-            using \<open>worldline t \<sigma> \<theta> \<tau> s k = signal_of2 (\<sigma> s) \<tau> s k\<close> 
+            using \<open>worldline t \<sigma> \<theta> \<tau> s k = signal_of2 (\<sigma> s) \<tau> s k\<close>
             \<open>worldline t \<sigma> \<theta> \<tau> s k = worldline t \<sigma> \<theta> \<tau> s t\<close> by blast }
-        ultimately show ?thesis by auto 
+        ultimately show ?thesis by auto
       qed
-      finally have "signal_of2 (\<sigma> s) (derivative_raw (worldline t \<sigma> \<theta> \<tau>) deg t) s k = 
+      finally have "signal_of2 (\<sigma> s) (derivative_raw (worldline t \<sigma> \<theta> \<tau>) deg t) s k =
                     signal_of2 (\<sigma> s) \<tau> s k"
         by auto }
-    ultimately have "signal_of2 (\<sigma> s) (derivative_raw (worldline t \<sigma> \<theta> \<tau>) deg t) s k = 
+    ultimately have "signal_of2 (\<sigma> s) (derivative_raw (worldline t \<sigma> \<theta> \<tau>) deg t) s k =
                     signal_of2 (\<sigma> s) \<tau> s k" by auto }
-  ultimately have "signal_of2 (\<sigma> s) (derivative_raw (worldline t \<sigma> \<theta> \<tau>) deg t) s k = 
+  ultimately have "signal_of2 (\<sigma> s) (derivative_raw (worldline t \<sigma> \<theta> \<tau>) deg t) s k =
                     signal_of2 (\<sigma> s) \<tau> s k" by auto
-  thus "signal_of2 (\<sigma> s) (derivative_raw (worldline t \<sigma> \<theta> \<tau>) (LEAST n. \<forall>ta>n. \<forall>s. worldline t \<sigma> \<theta> \<tau> s ta = worldline t \<sigma> \<theta> \<tau> s n) t) s k = 
+  thus "signal_of2 (\<sigma> s) (derivative_raw (worldline t \<sigma> \<theta> \<tau>) (LEAST n. \<forall>ta>n. \<forall>s. worldline t \<sigma> \<theta> \<tau> s ta = worldline t \<sigma> \<theta> \<tau> s n) t) s k =
         signal_of2 (\<sigma> s) \<tau> s k"
     unfolding deg_def by auto
 qed
 
-lemma destruct_worldline_correctness:               
+lemma destruct_worldline_correctness:
   assumes "context_invariant t \<sigma> \<gamma> \<theta> \<tau>"
   assumes "destruct_worldline (worldline2 t \<sigma> \<theta> \<tau>) t = (\<sigma>', \<gamma>', \<theta>', \<tau>')"
-  shows "\<sigma> = \<sigma>'" and "\<gamma> = \<gamma>'" 
+  shows "\<sigma> = \<sigma>'" and "\<gamma> = \<gamma>'"
     and "\<And>k s. signal_of2 False \<theta> s k = signal_of2 False \<theta>' s k"
     and "\<And>k s. signal_of2 (\<sigma> s) \<tau> s k = signal_of2 (\<sigma> s) \<tau>' s k"
   using assms(2) state_worldline2[OF assms(1)] event_worldline2[OF assms(1)] beh_of_worldline[OF assms(1)]
   transaction_worldline2[OF assms(1)] unfolding destruct_worldline_def Let_def by auto
 
 text \<open>Ideally, we want the destructor @{term "destruct_worldline"} is the inverse of the constructor
-@{term "worldline2"}. Unfortunately this is not the case here. Note that in the lemma above, 
-the states are the same @{term "\<sigma> = \<sigma>'"}, the events are the same @{term "\<gamma> = \<gamma>'"} but not with 
-the history (or behaviours) @{term "\<theta>"} @{term "\<theta>'"} and the transactions @{term "\<tau>"} @{term "\<tau>'"}. 
-Why is this the case? 
+@{term "worldline2"}. Unfortunately this is not the case here. Note that in the lemma above,
+the states are the same @{term "\<sigma> = \<sigma>'"}, the events are the same @{term "\<gamma> = \<gamma>'"} but not with
+the history (or behaviours) @{term "\<theta>"} @{term "\<theta>'"} and the transactions @{term "\<tau>"} @{term "\<tau>'"}.
+Why is this the case?
 
-To answer this question, we need to explain the ``inverse'' function of the derivative, i.e., 
-``integral'' which is achieved via the function @{term "signal_of2"}. It is basically the function 
-to turn a transaction into a signal. This ``integral'' function runs through over time, note if 
-there is a mapping, and change the signal value according to this mapping. It is basically like 
-integration function in real calculus, but the value can only either be ``0'' or ``1''. 
+To answer this question, we need to explain the ``inverse'' function of the derivative, i.e.,
+``integral'' which is achieved via the function @{term "signal_of2"}. It is basically the function
+to turn a transaction into a signal. This ``integral'' function runs through over time, note if
+there is a mapping, and change the signal value according to this mapping. It is basically like
+integration function in real calculus, but the value can only either be ``0'' or ``1''.
 
 The reason why we cannot have the equality @{term "\<tau> = \<tau>'"} and @{term "\<theta> = \<theta>'"} is because a
 worldline does not have a unique ``derivative''. Suppose that the transaction @{term "\<tau>"} maps the
@@ -753,16 +763,16 @@ that it also maps @{term "sig\<^sub>1 :: 'signal"} to @{term "True :: val"} at t
 ``integrate'' both of these transactions, we will obtain an identical worldline; posting (setting) a
 signal to @{term "True"} where we have previously posted (maps) the same value is futile.
 
-However, even though the transaction @{term "\<tau>'"} and history @{term "\<theta>"} are not guaranteed to be 
+However, even though the transaction @{term "\<tau>'"} and history @{term "\<theta>"} are not guaranteed to be
 the same with @{term "\<tau>"} and @{term "\<theta>"} any longer, the ``integrals'' are still the same; see
 property 3 and 4 in the theorem above.\<close>
 
-definition world_seq_exec :: "'signal worldline2 \<Rightarrow> nat \<Rightarrow> 'signal seq_stmt \<Rightarrow> 'signal worldline2" where 
-  "world_seq_exec w t s = (let (\<sigma>, \<gamma>, \<theta>, \<tau>) = destruct_worldline w t; 
-                                         \<tau>' = b_seq_exec t \<sigma> \<gamma> \<theta> s \<tau> 
+definition world_seq_exec :: "'signal worldline2 \<Rightarrow> nat \<Rightarrow> 'signal seq_stmt \<Rightarrow> 'signal worldline2" where
+  "world_seq_exec w t s = (let (\<sigma>, \<gamma>, \<theta>, \<tau>) = destruct_worldline w t;
+                                         \<tau>' = b_seq_exec t \<sigma> \<gamma> \<theta> s \<tau>
                            in worldline2 t \<sigma> \<theta> \<tau>')"
 
-abbreviation world_seq_exec_abb :: "'signal worldline2 \<Rightarrow> nat \<Rightarrow> 'signal seq_stmt \<Rightarrow> 'signal worldline2 \<Rightarrow> bool" 
+abbreviation world_seq_exec_abb :: "'signal worldline2 \<Rightarrow> nat \<Rightarrow> 'signal seq_stmt \<Rightarrow> 'signal worldline2 \<Rightarrow> bool"
   ("(_, _ , _) \<Rightarrow>\<^sub>s _")
   where "world_seq_exec_abb w t s w' \<equiv> (world_seq_exec w t s = w')"
 
@@ -780,8 +790,8 @@ definition
 seq_hoare_valid2 :: "nat \<Rightarrow> 'signal assn2 \<Rightarrow> 'signal seq_stmt \<Rightarrow> 'signal assn2 \<Rightarrow> bool" ("\<Turnstile>\<^sub>_ [(1_)]/ (_)/ [(1_)]" 50)
 where "\<Turnstile>\<^sub>t [P] s [Q] \<longleftrightarrow>  (\<forall>w w'.  P w \<and> (w, t, s \<Rightarrow>\<^sub>s w') \<longrightarrow> Q w')"
 
-text \<open>This is a cleaner definition of the validity compared to @{term "seq_hoare_valid"} in 
-@{theory "Draft.VHDL_Hoare"}. This also has the same spirit as the definition of validity in 
+text \<open>This is a cleaner definition of the validity compared to @{term "seq_hoare_valid"} in
+@{theory "Draft.VHDL_Hoare"}. This also has the same spirit as the definition of validity in
 @{theory_text "Hoare"}.\<close>
 
 lemma beval_cong:
@@ -795,7 +805,7 @@ lemma signal_of2_eq_is_stable:
   assumes "\<And>n. n < t \<Longrightarrow> lookup \<tau>1 n = 0"
   assumes "\<And>s. s \<in> dom (lookup \<tau>1 t) \<Longrightarrow> \<sigma> s = the (lookup \<tau>1 t s)"
   shows "is_stable dly \<tau>2 t sig (\<sigma> sig)"
-  unfolding is_stable_correct 
+  unfolding is_stable_correct
 proof safe
   fix m
   assume "t < m"
@@ -808,7 +818,7 @@ proof safe
   moreover
   { assume "lookup \<tau>2 m sig = Some x"
     hence "signal_of2 (\<sigma> sig) \<tau>2 sig m = x"
-      using lookup_some_signal_of2' by fastforce 
+      using lookup_some_signal_of2' by fastforce
     hence "signal_of2 (\<sigma> sig) \<tau>1 sig m = x"
       using assms(2) by auto
     have *: "lookup \<tau>1 m sig = None \<or> lookup \<tau>1 m sig = Some x"
@@ -867,22 +877,22 @@ proof safe
           using `lookup \<tau>2 m sig = Some x` by auto }
       moreover
       { assume "find (\<lambda>x. lookup \<tau>1 x sig \<noteq> None) (rev [0..< m]) = Some k"
-        hence " \<exists>i<length (rev [0..<m]). get_trans \<tau>1 (rev [0..<m] ! i) sig \<noteq> None 
-                                       \<and> k = rev [0..<m] ! i 
+        hence " \<exists>i<length (rev [0..<m]). get_trans \<tau>1 (rev [0..<m] ! i) sig \<noteq> None
+                                       \<and> k = rev [0..<m] ! i
                                        \<and> (\<forall>j<i. \<not> get_trans \<tau>1 (rev [0..<m] ! j) sig \<noteq> None)"
           unfolding find_Some_iff by auto
         then obtain i where "i<length (rev [0..<m])" and "get_trans \<tau>1 (rev [0..<m] ! i) sig \<noteq> None"
                       and "k = rev [0..<m] ! i " and quant: "\<forall>j<i.  lookup \<tau>1 (rev [0..<m] ! j) sig = None"
           by auto
-        have "k = m - i - 1" using `k = rev [0..<m] ! i` 
-          by (metis One_nat_def \<open>i < length (rev [0..<m])\<close> add.left_neutral add.right_neutral 
-              add_Suc_right diff_diff_add diff_less diff_zero length_rev length_upt nat_less_le 
+        have "k = m - i - 1" using `k = rev [0..<m] ! i`
+          by (metis One_nat_def \<open>i < length (rev [0..<m])\<close> add.left_neutral add.right_neutral
+              add_Suc_right diff_diff_add diff_less diff_zero length_rev length_upt nat_less_le
               neq0_conv nth_upt rev_nth zero_less_Suc zero_order(2))
         hence iless: "i < length ([0..<m])"
           using `i<length (rev [0..<m])` by auto
-        have "lookup \<tau>1 k sig \<noteq> None" 
+        have "lookup \<tau>1 k sig \<noteq> None"
           using rev_nth[OF iless] `lookup \<tau>1 (rev [0..<m] ! i) sig \<noteq> None` `k = m - i - 1`
-          using \<open>k = rev [0..<m] ! i\<close> by auto          
+          using \<open>k = rev [0..<m] ! i\<close> by auto
         have "\<And>j. j > k \<Longrightarrow>  j < m \<Longrightarrow> lookup \<tau>1 j sig = None"
         proof -
           fix j
@@ -905,7 +915,7 @@ proof safe
         qed
         hence ind: "\<And>j. k < j \<Longrightarrow> j \<le> m \<Longrightarrow> lookup \<tau>1 j sig = 0"
           using `lookup \<tau>1 m sig = None` using dual_order.order_iff_strict  zero_option_def by fastforce
-        have "t \<le> k" 
+        have "t \<le> k"
         proof (rule ccontr)
           assume "\<not> (t \<le> k)" hence "k < t" by auto
           hence "lookup \<tau>1 k sig = None"
@@ -937,16 +947,16 @@ proof safe
         moreover
         { assume "t < k"
           hence "x = \<sigma> sig"
-            using `lookup \<tau>1 k sig = Some x` assms(1) unfolding is_stable_correct 
+            using `lookup \<tau>1 k sig = Some x` assms(1) unfolding is_stable_correct
             using `t < k` `k < m` `m \<le> t + dly` by auto
           hence "check (lookup \<tau>2 m) sig (\<sigma> sig)"
             using `lookup \<tau>2 m sig = Some x` by auto }
         moreover
         { assume "t = k"
           hence "x = \<sigma> sig"
-            using assms(4) `lookup \<tau>1 k sig = Some x`  by (simp add: domIff) 
+            using assms(4) `lookup \<tau>1 k sig = Some x`  by (simp add: domIff)
           hence "check (lookup \<tau>2 m) sig (\<sigma> sig)"
-            using `lookup \<tau>2 m sig = Some x` by auto }          
+            using `lookup \<tau>2 m sig = Some x` by auto }
         ultimately have "check (lookup \<tau>2 m) sig (\<sigma> sig)"
           by auto }
       ultimately have "check (lookup \<tau>2 m) sig (\<sigma> sig)"
@@ -963,8 +973,8 @@ lemma signal_of2_eq_is_stable_eq:
   assumes "\<And>n. n < t \<Longrightarrow> lookup \<tau>2 n = 0"
   assumes "\<And>s. s \<in> dom (lookup \<tau>2 t) \<Longrightarrow> \<sigma> s = the (lookup \<tau>2 t s)"
   assumes "\<And>k s. signal_of2 (\<sigma> s) \<tau>1 s k = signal_of2 (\<sigma> s) \<tau>2 s k"
-  shows "is_stable dly \<tau>1 t sig (\<sigma> sig) \<longleftrightarrow> is_stable dly \<tau>2 t sig (\<sigma> sig)"  
-proof 
+  shows "is_stable dly \<tau>1 t sig (\<sigma> sig) \<longleftrightarrow> is_stable dly \<tau>2 t sig (\<sigma> sig)"
+proof
   assume "is_stable dly \<tau>1 t sig (\<sigma> sig)"
   with signal_of2_eq_is_stable[OF _ assms(5) assms(1-2)] show "is_stable dly \<tau>2 t sig (\<sigma> sig)"
     by auto
@@ -1012,7 +1022,7 @@ proof -
         finally have "lookup (purge dly \<tau>1 t sig (\<sigma> sig)) n = 0"
           by auto
         hence "n \<notin> dom (lookup (to_transaction2 (purge dly \<tau>1 t sig (\<sigma> sig)) sig))"
-          apply transfer' unfolding to_trans_raw2_def 
+          apply transfer' unfolding to_trans_raw2_def
           by (simp add: domIff zero_fun_def zero_option_def)
         with `n \<in> dom (lookup (to_transaction2 (purge dly \<tau>1 t sig (\<sigma> sig)) sig))`
         show False by auto
@@ -1041,12 +1051,12 @@ proof -
           hence " lookup (purge dly \<tau>1 t sig (\<sigma> sig)) n sig = lookup \<tau>1 n sig"
             using * by auto
           also have "... = 0"
-            using assms(2) `n \<le> t` `lookup \<tau>1 k sig = None` 
+            using assms(2) `n \<le> t` `lookup \<tau>1 k sig = None`
             by (metis \<open>k = t\<close> dual_order.order_iff_strict zero_fun_def zero_option_def)
           finally have "lookup (purge dly \<tau>1 t sig (\<sigma> sig)) n sig = 0"
             by auto
           hence "n \<notin> dom (lookup (to_transaction2 (purge dly \<tau>1 t sig (\<sigma> sig)) sig))"
-            apply transfer' unfolding to_trans_raw2_def 
+            apply transfer' unfolding to_trans_raw2_def
             by (simp add: domIff zero_fun_def zero_option_def)
           with `n \<in> dom (lookup (to_transaction2 (purge dly \<tau>1 t sig (\<sigma> sig)) sig))`
           show False by auto
@@ -1063,14 +1073,14 @@ proof -
       hence "lookup \<tau>1 k sig = Some (\<sigma> sig)"
         using `lookup \<tau>1 k sig = Some x` by auto
       hence ?thesis
-        using \<open>get_trans (purge dly \<tau>1 t sig (\<sigma> sig)) k sig = get_trans \<tau>1 k sig\<close> lookup_some_signal_of2' 
+        using \<open>get_trans (purge dly \<tau>1 t sig (\<sigma> sig)) k sig = get_trans \<tau>1 k sig\<close> lookup_some_signal_of2'
         by fastforce }
     ultimately have ?thesis by auto }
   moreover
-  { assume "t < k"  
-    have "lookup (purge dly \<tau>1 t sig (\<sigma> sig)) k sig = None \<or> 
+  { assume "t < k"
+    have "lookup (purge dly \<tau>1 t sig (\<sigma> sig)) k sig = None \<or>
           lookup (purge dly \<tau>1 t sig (\<sigma> sig)) k sig = Some (\<sigma> sig)"
-      by (simp add: \<open>t < k\<close> assms(1) order.strict_implies_order purge_correctness')    
+      by (simp add: \<open>t < k\<close> assms(1) order.strict_implies_order purge_correctness')
     moreover
     { assume "lookup (purge dly \<tau>1 t sig (\<sigma> sig)) k sig = Some (\<sigma> sig)"
       hence ?thesis
@@ -1088,7 +1098,7 @@ proof -
         hence "\<And>x. x < k \<Longrightarrow> lookup \<tau>1' x sig = None"
           by auto
         hence ***: "\<And>x. x \<le> k \<Longrightarrow> lookup \<tau>1' x sig = None"
-          using `lookup (purge dly \<tau>1 t sig (\<sigma> sig)) k sig = None` 
+          using `lookup (purge dly \<tau>1 t sig (\<sigma> sig)) k sig = None`
           unfolding \<tau>1'_def using nat_less_le by blast
         have "signal_of2 (\<sigma> sig) \<tau>1' sig k = \<sigma> sig"
         proof -
@@ -1113,20 +1123,20 @@ proof -
           unfolding \<tau>1'_def by auto }
       moreover
       { assume "find (\<lambda>x. lookup \<tau>1' x sig \<noteq> None) (rev [0..< k]) = Some k'"
-        hence " \<exists>i<length (rev [0..<k]). get_trans \<tau>1' (rev [0..<k] ! i) sig \<noteq> None 
-                                       \<and> k' = rev [0..<k] ! i 
+        hence " \<exists>i<length (rev [0..<k]). get_trans \<tau>1' (rev [0..<k] ! i) sig \<noteq> None
+                                       \<and> k' = rev [0..<k] ! i
                                        \<and> (\<forall>j<i. \<not> get_trans \<tau>1' (rev [0..<k] ! j) sig \<noteq> None)"
           unfolding find_Some_iff by auto
         then obtain i where "i<length (rev [0..<k])" and "get_trans \<tau>1' (rev [0..<k] ! i) sig \<noteq> None"
                       and "k' = rev [0..<k] ! i " and quant: "\<forall>j<i.  lookup \<tau>1' (rev [0..<k] ! j) sig = None"
           by auto
-        have "k' = k - i - 1" using `k' = rev [0..<k] ! i` 
-          by (metis One_nat_def \<open>i < length (rev [0..<k])\<close> add.left_neutral add.right_neutral 
-              add_Suc_right diff_diff_add diff_less diff_zero length_rev length_upt nat_less_le 
+        have "k' = k - i - 1" using `k' = rev [0..<k] ! i`
+          by (metis One_nat_def \<open>i < length (rev [0..<k])\<close> add.left_neutral add.right_neutral
+              add_Suc_right diff_diff_add diff_less diff_zero length_rev length_upt nat_less_le
               neq0_conv nth_upt rev_nth zero_less_Suc zero_order(2))
         hence iless: "i < length ([0..<k])"
           using `i<length (rev [0..<k])` by auto
-        have "lookup \<tau>1' k' sig \<noteq> None" 
+        have "lookup \<tau>1' k' sig \<noteq> None"
           using rev_nth[OF iless] `lookup \<tau>1' (rev [0..<k] ! i) sig \<noteq> None` `k' = k - i - 1`
           using \<open>k' = rev [0..<k] ! i\<close> by auto
         have "\<And>j. j > k' \<Longrightarrow>  j < k \<Longrightarrow> lookup \<tau>1' j sig = None"
@@ -1150,7 +1160,7 @@ proof -
             using nth_upt `j < k` by auto
         qed
         hence ind: "\<And>j. k' < j \<Longrightarrow> j \<le> k \<Longrightarrow> lookup \<tau>1' j sig = 0"
-          using `lookup (purge dly \<tau>1 t sig (\<sigma> sig)) k sig = None` unfolding \<tau>1'_def 
+          using `lookup (purge dly \<tau>1 t sig (\<sigma> sig)) k sig = None` unfolding \<tau>1'_def
           using dual_order.order_iff_strict  zero_option_def by fastforce
         have "k' < k"
           using \<open>i < length (rev [0..<k])\<close> \<open>k' = k - i - 1\<close> by auto
@@ -1208,11 +1218,11 @@ proof -
                 then obtain n where "n \<in> dom (lookup (to_transaction2 \<tau>1' sig))" and "n \<le> k"
                   using \<open>get_trans \<tau>1' k' sig = None\<close> \<open>get_trans \<tau>1' k' sig \<noteq> None\<close> by blast
                 have "lookup \<tau>1' n sig = None"
-                  using `n \<le> k` ** `lookup \<tau>1' k' sig = None` `t = k'` unfolding \<tau>1'_def 
+                  using `n \<le> k` ** `lookup \<tau>1' k' sig = None` `t = k'` unfolding \<tau>1'_def
                   using \<open>get_trans \<tau>1' k' sig \<noteq> None\<close> \<tau>1'_def by blast
                 hence "n \<notin> dom (lookup (to_transaction2 \<tau>1' sig))"
-                  by (transfer', auto simp add:to_trans_raw2_def) 
-                with `n \<in> dom (lookup (to_transaction2 \<tau>1' sig))` show False 
+                  by (transfer', auto simp add:to_trans_raw2_def)
+                with `n \<in> dom (lookup (to_transaction2 \<tau>1' sig))` show False
                   by auto
               qed
               hence "inf_time (to_transaction2 \<tau>1') sig k = None "
@@ -1228,7 +1238,7 @@ proof -
     ultimately have ?thesis by auto }
   ultimately show ?thesis by auto
 qed
-         
+
 lemma helper':
   assumes "t, \<sigma>, \<gamma>, \<theta>1 \<turnstile> <ss, \<tau>1> \<longrightarrow>\<^sub>s \<tau>1'"
   assumes "\<And>k s. signal_of2 False \<theta>1 s k = signal_of2 False \<theta>2 s k"
@@ -1247,11 +1257,11 @@ proof (induction ss arbitrary:\<tau>1 \<tau>2 \<tau>1' \<tau>2')
   have "\<And>k s. signal_of2 (\<sigma> s) \<tau> s k = signal_of2 (\<sigma> s) \<tau>' s k"
     using Bcomp(1)[OF tau1 Bcomp(4) Bcomp(5) tau3 Bcomp(7-8) `nonneg_delay ss1`] by auto
   moreover have "context_invariant t \<sigma> \<gamma> \<theta>1 \<tau>"
-    using b_seq_exec_preserves_context_invariant[OF Bcomp(7) tau1 `nonneg_delay ss1`] 
+    using b_seq_exec_preserves_context_invariant[OF Bcomp(7) tau1 `nonneg_delay ss1`]
     by auto
   moreover have "context_invariant t \<sigma> \<gamma> \<theta>2 \<tau>'"
     using b_seq_exec_preserves_context_invariant[OF Bcomp(8) tau3 `nonneg_delay ss1`] .
-  ultimately show ?case 
+  ultimately show ?case
     using Bcomp(2)[OF tau2 Bcomp(4) _ tau4] `nonneg_delay ss2` by auto
 next
   case (Bguarded g ss1 ss2)
@@ -1268,7 +1278,7 @@ next
     hence "\<tau>2' = b_seq_exec t \<sigma> \<gamma> \<theta>2 ss1 \<tau>2"
       using Bguarded(6) by auto
     hence ?case
-      using Bguarded(1) `\<tau>1' = b_seq_exec t \<sigma> \<gamma> \<theta>1 ss1 \<tau>1` Bguarded(4-5) 
+      using Bguarded(1) `\<tau>1' = b_seq_exec t \<sigma> \<gamma> \<theta>1 ss1 \<tau>1` Bguarded(4-5)
       Bguarded.prems(5) Bguarded.prems(6) \<open>nonneg_delay ss1\<close> by blast }
   moreover
   { assume "\<not> beval t \<sigma> \<gamma> \<theta>1 g"
@@ -1276,9 +1286,9 @@ next
       using beval_cong[OF Bguarded(4)] by auto
     hence "\<tau>1' = b_seq_exec t \<sigma> \<gamma> \<theta>1 ss2 \<tau>1" and "\<tau>2' = b_seq_exec t \<sigma> \<gamma> \<theta>2 ss2 \<tau>2"
       using `\<not> beval t \<sigma> \<gamma> \<theta>1 g` using Bguarded by auto
-    hence ?case 
+    hence ?case
       using Bguarded \<open>nonneg_delay ss2\<close> by blast }
-  ultimately show ?case 
+  ultimately show ?case
     by auto
 next
   case (Bassign_trans sig e dly)
@@ -1366,7 +1376,7 @@ next
     have ci2: "\<And>n. n < t \<Longrightarrow> lookup \<tau>2 n = 0" and ci3: "\<And>s. s \<in> dom (lookup \<tau>2 t) \<Longrightarrow> \<sigma> s = the (lookup \<tau>2 t s)"
       using `context_invariant t \<sigma> \<gamma> \<theta>2 \<tau>2` unfolding context_invariant_def by auto
     have nstable2: "\<not> is_stable dly \<tau>2 t sig (\<sigma> sig)"
-      using signal_of2_eq_is_stable_eq[OF ci0 ci1 ci2 ci3 Bassign_inert(3)] 
+      using signal_of2_eq_is_stable_eq[OF ci0 ci1 ci2 ci3 Bassign_inert(3)]
       `\<not> is_stable dly \<tau>1 t sig (\<sigma> sig)` by auto
     have tau1': "\<tau>1' = trans_post sig x (purge dly \<tau>1 t sig (\<sigma> sig)) (t + dly)"
       using tau1 nstable1 unfolding inr_post_def by auto
@@ -1383,7 +1393,7 @@ next
     moreover have "s \<noteq> sig \<Longrightarrow> signal_of2 (\<sigma> s) \<tau>2 s k = signal_of2 (\<sigma> s) (purge dly \<tau>2 t sig (\<sigma> sig)) s k"
       using signal_of2_purge_not_affected by fastforce
     ultimately have *: "s \<noteq> sig \<Longrightarrow> signal_of2 (\<sigma> s) \<tau>1' s k = signal_of2 (\<sigma> s) \<tau>2' s k"
-      using signal_of_trans_post unfolding tau2' by metis    
+      using signal_of_trans_post unfolding tau2' by metis
     have "t + dly \<le> k \<or> k < t + dly"
       by auto
     moreover
@@ -1424,7 +1434,7 @@ lemma helper:
   assumes "context_invariant t \<sigma> \<gamma> \<theta>1 \<tau>1" and "context_invariant t \<sigma> \<gamma> \<theta>2 \<tau>2"
   assumes "nonneg_delay ss"
   shows "\<exists>\<tau>2'. (t, \<sigma>, \<gamma>, \<theta>2 \<turnstile> <ss, \<tau>2> \<longrightarrow>\<^sub>s \<tau>2') \<and> (\<forall>k s. signal_of2 (\<sigma> s) \<tau>1' s k = signal_of2 (\<sigma> s) \<tau>2' s k)"
-  using helper'[OF assms(1-3) _ assms(4-5) `nonneg_delay ss`] by auto 
+  using helper'[OF assms(1-3) _ assms(4-5) `nonneg_delay ss`] by auto
 
 lemma Bcomp_hoare_valid':
   assumes "\<Turnstile>\<^sub>t [P] s1 [Q]" and "\<Turnstile>\<^sub>t [Q] s2 [R]"
@@ -1437,7 +1447,7 @@ proof (rule)+
     using assms(3) by auto
   assume "P w \<and> (w, t, Bcomp s1 s2 \<Rightarrow>\<^sub>s w')"
   hence "P w" and "w, t, Bcomp s1 s2 \<Rightarrow>\<^sub>s w'" by auto
-  then obtain \<sigma> \<gamma> \<theta> \<tau> \<tau>' where des: "destruct_worldline w t = (\<sigma>, \<gamma>, \<theta>, \<tau>)" and 
+  then obtain \<sigma> \<gamma> \<theta> \<tau> \<tau>' where des: "destruct_worldline w t = (\<sigma>, \<gamma>, \<theta>, \<tau>)" and
     "(t, \<sigma>, \<gamma>, \<theta> \<turnstile> <Bcomp s1 s2, \<tau>> \<longrightarrow>\<^sub>s \<tau>')" and "w'= worldline2 t \<sigma> \<theta> \<tau>'"
     unfolding world_seq_exec_def Let_def using destruct_worldline_exist by fastforce
   then obtain \<tau>'' where tau1: "(t, \<sigma>, \<gamma>, \<theta> \<turnstile> <s1, \<tau>> \<longrightarrow>\<^sub>s \<tau>'')" and tau2: "(t, \<sigma>, \<gamma>, \<theta> \<turnstile> <s2, \<tau>''> \<longrightarrow>\<^sub>s \<tau>')"
@@ -1445,16 +1455,16 @@ proof (rule)+
   define w'' where "w'' = worldline2 t \<sigma> \<theta> \<tau>''"
   hence "w, t, s1 \<Rightarrow>\<^sub>s w''"
     using des tau1 unfolding world_seq_exec_def Let_def by auto
-  with assms(1) have "Q w''" 
+  with assms(1) have "Q w''"
     unfolding seq_hoare_valid2_def using `P w` by auto
   have "context_invariant t \<sigma> \<gamma> \<theta> \<tau>"
     using worldline2_constructible[OF des] by auto
   hence "context_invariant t \<sigma> \<gamma> \<theta> \<tau>''"
     using b_seq_exec_preserves_context_invariant[OF _ tau1] assms(3) by auto
-  obtain \<theta>''' \<tau>''' where des2: "destruct_worldline w'' t = (\<sigma>, \<gamma>, \<theta>''', \<tau>''')" and 
-    sig_beh: "\<And>k s. signal_of2 False \<theta> s k = signal_of2 False \<theta>''' s k" and 
+  obtain \<theta>''' \<tau>''' where des2: "destruct_worldline w'' t = (\<sigma>, \<gamma>, \<theta>''', \<tau>''')" and
+    sig_beh: "\<And>k s. signal_of2 False \<theta> s k = signal_of2 False \<theta>''' s k" and
     sig_trans: "\<And>k s. signal_of2 (\<sigma> s) \<tau>'' s k = signal_of2 (\<sigma> s) \<tau>''' s k"
-    unfolding w''_def using destruct_worldline_correctness[OF `context_invariant t \<sigma> \<gamma> \<theta> \<tau>''`]   
+    unfolding w''_def using destruct_worldline_correctness[OF `context_invariant t \<sigma> \<gamma> \<theta> \<tau>''`]
     by (metis destruct_worldline_exist)
   have "context_invariant t \<sigma> \<gamma> \<theta>''' \<tau>'''"
     using worldline2_constructible[OF des2] by auto
@@ -1464,8 +1474,8 @@ proof (rule)+
   have "worldline2 t \<sigma> \<theta> \<tau>' = worldline2 t \<sigma> \<theta>''' \<tau>4"
     using sig_beh sig_trans
   proof transfer'
-    fix \<theta>  \<theta>''' :: "'a transaction" 
-    fix \<sigma> :: "'a state" 
+    fix \<theta>  \<theta>''' :: "'a transaction"
+    fix \<sigma> :: "'a state"
     fix \<tau>'' \<tau>''' \<tau>4 t \<tau>'
     assume 1: "\<And>s k. signal_of2 False \<theta> s k = signal_of2 False \<theta>''' s k"
     assume  "\<And>s k. signal_of2 (\<sigma> s) \<tau>4 s k = signal_of2 (\<sigma> s) \<tau>' s k"
@@ -1477,10 +1487,10 @@ proof (rule)+
   with `Q w''` show "R w'"
     using assms(2) unfolding seq_hoare_valid2_def by auto
 qed
-  
+
 lemma Bnull_sound_hoare2:
   "\<turnstile>\<^sub>t [P] Bnull [Q] \<Longrightarrow> \<Turnstile>\<^sub>t [P] Bnull [Q]"
-  by (auto dest!: BnullE'_hoare2 worldline2_constructible  simp add: seq_hoare_valid2_def world_seq_exec_def  
+  by (auto dest!: BnullE'_hoare2 worldline2_constructible  simp add: seq_hoare_valid2_def world_seq_exec_def
       split: prod.splits)
 
 lemma Bguarded_hoare_valid2:
@@ -1498,7 +1508,7 @@ proof (rule)+
   obtain \<tau>' where "t , \<sigma> , \<gamma> , \<theta> \<turnstile> <Bguarded g s1 s2, \<tau>> \<longrightarrow>\<^sub>s \<tau>'"
     by auto
   hence "w' = worldline2 t \<sigma> \<theta> \<tau>'"
-    using `w, t, Bguarded g s1 s2 \<Rightarrow>\<^sub>s w'` `destruct_worldline w t = (\<sigma>, \<gamma>, \<theta>, \<tau>)` 
+    using `w, t, Bguarded g s1 s2 \<Rightarrow>\<^sub>s w'` `destruct_worldline w t = (\<sigma>, \<gamma>, \<theta>, \<tau>)`
     unfolding world_seq_exec_def by auto
   have "beval t \<sigma> \<gamma> \<theta> g \<or> \<not> beval t \<sigma> \<gamma> \<theta> g"
     by auto
@@ -1511,7 +1521,7 @@ proof (rule)+
       by (transfer', simp add: beval_beval_world_ci)
     have "w, t , s1 \<Rightarrow>\<^sub>s w'"
       using `destruct_worldline w t = (\<sigma>, \<gamma>, \<theta>, \<tau>)` `t, \<sigma>, \<gamma>, \<theta> \<turnstile> <s1, \<tau>> \<longrightarrow>\<^sub>s \<tau>'`
-      `w' = worldline2 t \<sigma> \<theta> \<tau>'` unfolding world_seq_exec_def Let_def by auto 
+      `w' = worldline2 t \<sigma> \<theta> \<tau>'` unfolding world_seq_exec_def Let_def by auto
     with assms(1) and `P w` have "Q w'"
       using `beval_world2 w t g` unfolding seq_hoare_valid2_def by auto }
   moreover
@@ -1523,7 +1533,7 @@ proof (rule)+
       by (transfer', simp add: beval_beval_world_ci)
     have "w, t, s2 \<Rightarrow>\<^sub>s w'"
       using `destruct_worldline w t = (\<sigma>, \<gamma>, \<theta>, \<tau>)` `t, \<sigma>, \<gamma>, \<theta> \<turnstile> <s2, \<tau>> \<longrightarrow>\<^sub>s \<tau>'`
-      `w' = worldline2 t \<sigma> \<theta> \<tau>'` unfolding world_seq_exec_def Let_def by auto     
+      `w' = worldline2 t \<sigma> \<theta> \<tau>'` unfolding world_seq_exec_def Let_def by auto
     with assms(2) and `P w` have "Q w'"
       using `\<not> beval_world2 w t g` unfolding seq_hoare_valid2_def by auto }
   ultimately show "Q w'"
@@ -1533,10 +1543,10 @@ qed
 lemma lift_world_trans_worldline_upd2:
   assumes "w, t, Bassign_trans sig exp dly \<Rightarrow>\<^sub>s w'"
   shows "w' = w[sig, t + dly :=\<^sub>2 beval_world2 w t exp]"
-  using assms 
+  using assms
 proof transfer'
-  fix w t sig 
-  fix exp :: "'a bexp" 
+  fix w t sig
+  fix exp :: "'a bexp"
   fix dly w'
   assume "w, t , Bassign_trans sig exp dly \<Rightarrow>\<^sub>s w'"
   obtain \<sigma> \<gamma> \<theta> \<tau> where "destruct_worldline w t = (\<sigma>, \<gamma>, \<theta>, \<tau>)"
@@ -1552,15 +1562,15 @@ proof transfer'
   ultimately have \<tau>'_def: "\<tau>' = trans_post sig (beval_world2 w t exp) \<tau> (t + dly)"
       by auto
   have "w' = worldline2 t \<sigma> \<theta> \<tau>'"
-    using `w, t , Bassign_trans sig exp dly \<Rightarrow>\<^sub>s w'` `destruct_worldline w t = (\<sigma>, \<gamma>, \<theta>, \<tau>)` 
-    unfolding world_seq_exec_def  using \<open>t , \<sigma> , \<gamma> , \<theta> \<turnstile> <Bassign_trans sig exp dly , \<tau>> \<longrightarrow>\<^sub>s \<tau>'\<close> 
+    using `w, t , Bassign_trans sig exp dly \<Rightarrow>\<^sub>s w'` `destruct_worldline w t = (\<sigma>, \<gamma>, \<theta>, \<tau>)`
+    unfolding world_seq_exec_def  using \<open>t , \<sigma> , \<gamma> , \<theta> \<turnstile> <Bassign_trans sig exp dly , \<tau>> \<longrightarrow>\<^sub>s \<tau>'\<close>
     by auto
   also have "... = w[sig, t + dly:=\<^sub>2 beval_world2 w t exp]"
     using w_def \<tau>'_def by (transfer', meson lift_trans_post_worldline_upd)
   finally show "w' = w[sig, t + dly:=\<^sub>2 beval_world2 w t exp]"
     by auto
 qed
-  
+
 lemma Bassign_trans_sound_hoare2:
   "\<turnstile>\<^sub>t [P] Bassign_trans sig exp dly [Q] \<Longrightarrow> \<Turnstile>\<^sub>t [P] Bassign_trans sig exp dly [Q]"
   unfolding seq_hoare_valid2_def
@@ -1576,28 +1586,28 @@ proof rule+
   obtain \<tau>' where "t , \<sigma> , \<gamma> , \<theta> \<turnstile> <Bassign_trans sig exp dly, \<tau>> \<longrightarrow>\<^sub>s \<tau>'"
     by auto
   hence "w' = worldline2 t \<sigma> \<theta> \<tau>'"
-    using `w, t , Bassign_trans sig exp dly \<Rightarrow>\<^sub>s w'` `destruct_worldline w t = (\<sigma>, \<gamma>, \<theta>, \<tau>)` 
-    unfolding world_seq_exec_def  using \<open>t , \<sigma> , \<gamma> , \<theta> \<turnstile> <Bassign_trans sig exp dly , \<tau>> \<longrightarrow>\<^sub>s \<tau>'\<close> by auto  
+    using `w, t , Bassign_trans sig exp dly \<Rightarrow>\<^sub>s w'` `destruct_worldline w t = (\<sigma>, \<gamma>, \<theta>, \<tau>)`
+    unfolding world_seq_exec_def  using \<open>t , \<sigma> , \<gamma> , \<theta> \<turnstile> <Bassign_trans sig exp dly , \<tau>> \<longrightarrow>\<^sub>s \<tau>'\<close> by auto
   have "w' = w[sig, t + dly :=\<^sub>2 beval_world2 w t exp]"
-    unfolding `w' = worldline2 t \<sigma> \<theta> \<tau>'` 
-    by (simp add: \<open>w' = worldline2 t \<sigma> \<theta> \<tau>'\<close> \<open>w, t , Bassign_trans sig exp dly \<Rightarrow>\<^sub>s w'\<close> lift_world_trans_worldline_upd2) 
+    unfolding `w' = worldline2 t \<sigma> \<theta> \<tau>'`
+    by (simp add: \<open>w' = worldline2 t \<sigma> \<theta> \<tau>'\<close> \<open>w, t , Bassign_trans sig exp dly \<Rightarrow>\<^sub>s w'\<close> lift_world_trans_worldline_upd2)
   with imp and `P w` have "Q(w[sig, t + dly :=\<^sub>2 beval_world2 w t exp])"
-    by auto 
+    by auto
   thus "Q w'"
     using `Q(w[sig, t + dly :=\<^sub>2 beval_world2 w t exp])` `w' = w[sig, t + dly :=\<^sub>2 beval_world2 w t exp]`
     by auto
 qed
- 
+
 lemma lift_world_inert_worldline_upd2:
   assumes "w, t, Bassign_inert sig exp dly \<Rightarrow>\<^sub>s w'"
   assumes "0 < dly"
   shows "w' = w[sig, t, dly :=\<^sub>2 beval_world2 w t exp]"
   using assms
 proof transfer'
-  fix w t sig 
-  fix exp :: "'a bexp" 
+  fix w t sig
+  fix exp :: "'a bexp"
   fix dly w'
-  assume "w, t , Bassign_inert sig exp dly \<Rightarrow>\<^sub>s w'"  
+  assume "w, t , Bassign_inert sig exp dly \<Rightarrow>\<^sub>s w'"
   assume "0 < dly"
   obtain \<sigma> \<gamma> \<theta> \<tau> where "destruct_worldline w t = (\<sigma>, \<gamma>, \<theta>, \<tau>)"
     by (meson destruct_worldline_def)
@@ -1612,8 +1622,8 @@ proof transfer'
   ultimately have \<tau>'_def: "\<tau>' = inr_post sig (beval_world2 w t exp) (\<sigma> sig) \<tau> t dly"
     by auto
   have "w' = worldline2 t \<sigma> \<theta> \<tau>'"
-    using `w, t , Bassign_inert sig exp dly \<Rightarrow>\<^sub>s w'` `destruct_worldline w t = (\<sigma>, \<gamma>, \<theta>, \<tau>)` 
-    unfolding world_seq_exec_def  using \<open>t , \<sigma> , \<gamma> , \<theta> \<turnstile> <Bassign_inert sig exp dly , \<tau>> \<longrightarrow>\<^sub>s \<tau>'\<close> 
+    using `w, t , Bassign_inert sig exp dly \<Rightarrow>\<^sub>s w'` `destruct_worldline w t = (\<sigma>, \<gamma>, \<theta>, \<tau>)`
+    unfolding world_seq_exec_def  using \<open>t , \<sigma> , \<gamma> , \<theta> \<turnstile> <Bassign_inert sig exp dly , \<tau>> \<longrightarrow>\<^sub>s \<tau>'\<close>
     by auto
   also have "... = w[sig, t, dly:=\<^sub>2 beval_world2 w t exp]"
     using `w = worldline2 t \<sigma> \<theta> \<tau>` `context_invariant t \<sigma> \<gamma> \<theta> \<tau>`
@@ -1639,15 +1649,15 @@ proof rule+
   obtain \<tau>' where "t , \<sigma> , \<gamma> , \<theta> \<turnstile> <Bassign_inert sig exp dly, \<tau>> \<longrightarrow>\<^sub>s \<tau>'"
     by auto
   hence "w' = worldline2 t \<sigma> \<theta> \<tau>'"
-    using `w, t , Bassign_inert sig exp dly \<Rightarrow>\<^sub>s w'` `destruct_worldline w t = (\<sigma>, \<gamma>, \<theta>, \<tau>)` 
-    unfolding world_seq_exec_def  using \<open>t , \<sigma> , \<gamma> , \<theta> \<turnstile> <Bassign_inert sig exp dly , \<tau>> \<longrightarrow>\<^sub>s \<tau>'\<close> by auto  
+    using `w, t , Bassign_inert sig exp dly \<Rightarrow>\<^sub>s w'` `destruct_worldline w t = (\<sigma>, \<gamma>, \<theta>, \<tau>)`
+    unfolding world_seq_exec_def  using \<open>t , \<sigma> , \<gamma> , \<theta> \<turnstile> <Bassign_inert sig exp dly , \<tau>> \<longrightarrow>\<^sub>s \<tau>'\<close> by auto
   have "w' = w[sig, t, dly :=\<^sub>2 beval_world2 w t exp]"
     by (simp add: \<open>w, t , Bassign_inert sig exp dly \<Rightarrow>\<^sub>s w'\<close> assms lift_world_inert_worldline_upd2)
   with imp and `P w` have "Q(w[sig, t, dly :=\<^sub>2 beval_world2 w t exp])"
-    by auto 
+    by auto
   thus "Q w'"
     using `Q(w[sig, t,  dly :=\<^sub>2 beval_world2 w t exp])` `w' = w[sig, t, dly :=\<^sub>2 beval_world2 w t exp]`
-    by auto 
+    by auto
 qed
 
 subsection \<open>Soundness and completeness\<close>
@@ -1670,14 +1680,14 @@ qed (auto simp add: Bnull_sound_hoare2 Bassign_trans_sound_hoare2 Bcomp_hoare_va
 lemma  world_seq_exec_bnull:
   "w, t, Bnull \<Rightarrow>\<^sub>s w"
   unfolding world_seq_exec_def Let_def
-  by (metis (mono_tags, lifting) b_seq_exec.simps(1) destruct_worldline_exist old.prod.case 
+  by (metis (mono_tags, lifting) b_seq_exec.simps(1) destruct_worldline_exist old.prod.case
       worldline2_constructible)
 
 lemma world_seq_exec_comp:
   assumes "nonneg_delay (Bcomp ss1 ss2)"
   shows "w, t, (Bcomp ss1 ss2) \<Rightarrow>\<^sub>s (world_seq_exec (world_seq_exec w t ss1) t ss2)"
 proof -
-  obtain \<sigma> \<gamma> \<theta> \<tau> \<tau>' where des1: "destruct_worldline w t = (\<sigma>, \<gamma>, \<theta>, \<tau>)" and 
+  obtain \<sigma> \<gamma> \<theta> \<tau> \<tau>' where des1: "destruct_worldline w t = (\<sigma>, \<gamma>, \<theta>, \<tau>)" and
     "t, \<sigma>, \<gamma>, \<theta> \<turnstile> <Bcomp ss1 ss2, \<tau>> \<longrightarrow>\<^sub>s \<tau>'" and ci1: "context_invariant t \<sigma> \<gamma> \<theta> \<tau>"
     using destruct_worldline_exist worldline2_constructible by blast
   then obtain \<tau>'' where "t, \<sigma>, \<gamma>, \<theta> \<turnstile> <ss1, \<tau>> \<longrightarrow>\<^sub>s \<tau>''" and exec1: "t, \<sigma>, \<gamma>, \<theta> \<turnstile> <ss2, \<tau>''> \<longrightarrow>\<^sub>s \<tau>'"
@@ -1686,21 +1696,21 @@ proof -
   hence *: "worldline2 t \<sigma> \<theta> \<tau>'' = world_seq_exec w t ss1"
     unfolding world_seq_exec_def Let_def using des1 by auto
 
-  obtain \<theta>2 \<tau>2 \<tau>3 where des2: "destruct_worldline (worldline2 t \<sigma> \<theta> \<tau>'') t = (\<sigma>, \<gamma>, \<theta>2, \<tau>2)" and 
-    beh_same:"\<And>s k. signal_of2 False \<theta> s k = signal_of2 False \<theta>2 s k" and 
-    trans_same: "\<And>s k. signal_of2 (\<sigma> s) \<tau>'' s k = signal_of2 (\<sigma> s) \<tau>2 s k" and 
-    exec2: "t, \<sigma>, \<gamma>, \<theta>2 \<turnstile> <ss2, \<tau>2> \<longrightarrow>\<^sub>s \<tau>3" 
+  obtain \<theta>2 \<tau>2 \<tau>3 where des2: "destruct_worldline (worldline2 t \<sigma> \<theta> \<tau>'') t = (\<sigma>, \<gamma>, \<theta>2, \<tau>2)" and
+    beh_same:"\<And>s k. signal_of2 False \<theta> s k = signal_of2 False \<theta>2 s k" and
+    trans_same: "\<And>s k. signal_of2 (\<sigma> s) \<tau>'' s k = signal_of2 (\<sigma> s) \<tau>2 s k" and
+    exec2: "t, \<sigma>, \<gamma>, \<theta>2 \<turnstile> <ss2, \<tau>2> \<longrightarrow>\<^sub>s \<tau>3"
     using destruct_worldline_correctness[OF ci2]  by (metis prod.exhaust_sel)
   have ci3: "context_invariant t \<sigma> \<gamma> \<theta>2 \<tau>2"
     using worldline2_constructible[OF des2] by auto
   have "\<And>s k. signal_of2 (\<sigma> s) \<tau>' s k = signal_of2 (\<sigma> s) \<tau>3 s k"
     using helper'[OF exec1 beh_same trans_same exec2 ci2 ci3] assms by auto
   hence "worldline2 t \<sigma> \<theta> \<tau>' = worldline2 t \<sigma> \<theta>2 \<tau>3"
-    using beh_same 
+    using beh_same
   proof (transfer')
     fix \<sigma> :: "'a state"
-    fix \<tau>' \<tau>3 
-    fix \<theta> \<theta>2 :: "'a transaction" 
+    fix \<tau>' \<tau>3
+    fix \<theta> \<theta>2 :: "'a transaction"
     fix t
     assume 1: "\<And>s k. signal_of2 (\<sigma> s) \<tau>' s k = signal_of2 (\<sigma> s) \<tau>3 s k"
     assume "\<And>s k. signal_of2 False \<theta> s k = signal_of2 False \<theta>2 s k"
@@ -1708,7 +1718,7 @@ proof -
       unfolding worldline_def  using 1 by auto
   qed
   also have "... = world_seq_exec (worldline2 t \<sigma> \<theta> \<tau>'') t ss2"
-    using des2 `t, \<sigma>, \<gamma>, \<theta>2 \<turnstile> <ss2, \<tau>2> \<longrightarrow>\<^sub>s \<tau>3` unfolding world_seq_exec_def Let_def 
+    using des2 `t, \<sigma>, \<gamma>, \<theta>2 \<turnstile> <ss2, \<tau>2> \<longrightarrow>\<^sub>s \<tau>3` unfolding world_seq_exec_def Let_def
     by auto
   finally have "worldline2 t \<sigma> \<theta> \<tau>' = world_seq_exec (worldline2 t \<sigma> \<theta> \<tau>'') t ss2"
     by auto
@@ -1721,15 +1731,15 @@ lemma world_seq_exec_guarded:
   assumes "beval_world2 w t g"
   shows "world_seq_exec w t (Bguarded g ss1 ss2) = world_seq_exec w t ss1"
 proof -
-  obtain \<sigma> \<gamma> \<theta> \<tau> \<tau>' where des1: "destruct_worldline w t = (\<sigma>, \<gamma>, \<theta>, \<tau>)" and 
-    "t, \<sigma>, \<gamma>, \<theta> \<turnstile> <Bguarded g ss1 ss2, \<tau>> \<longrightarrow>\<^sub>s \<tau>'" and ci1: "context_invariant t \<sigma> \<gamma> \<theta> \<tau>" and 
+  obtain \<sigma> \<gamma> \<theta> \<tau> \<tau>' where des1: "destruct_worldline w t = (\<sigma>, \<gamma>, \<theta>, \<tau>)" and
+    "t, \<sigma>, \<gamma>, \<theta> \<turnstile> <Bguarded g ss1 ss2, \<tau>> \<longrightarrow>\<^sub>s \<tau>'" and ci1: "context_invariant t \<sigma> \<gamma> \<theta> \<tau>" and
     "w = worldline2 t \<sigma> \<theta> \<tau>" using destruct_worldline_exist worldline2_constructible by blast
   moreover have "beval t \<sigma> \<gamma> \<theta> g"
     using assms `w = worldline2 t \<sigma> \<theta> \<tau>` ci1  apply transfer' using beval_beval_world_ci by metis
   ultimately have "t, \<sigma>, \<gamma>, \<theta> \<turnstile> <ss1, \<tau>> \<longrightarrow>\<^sub>s \<tau>'"
     by auto
   thus ?thesis
-    by (metis (no_types, lifting) \<open>t , \<sigma> , \<gamma> , \<theta> \<turnstile> <Bguarded g ss1 ss2 , \<tau>> \<longrightarrow>\<^sub>s \<tau>'\<close> case_prod_conv 
+    by (metis (no_types, lifting) \<open>t , \<sigma> , \<gamma> , \<theta> \<turnstile> <Bguarded g ss1 ss2 , \<tau>> \<longrightarrow>\<^sub>s \<tau>'\<close> case_prod_conv
         des1 world_seq_exec_def)
 qed
 
@@ -1737,22 +1747,22 @@ lemma world_seq_exec_guarded_not:
   assumes "\<not> beval_world2 w t g"
   shows "world_seq_exec w t (Bguarded g ss1 ss2) = world_seq_exec w t ss2"
 proof -
-  obtain \<sigma> \<gamma> \<theta> \<tau> \<tau>' where des1: "destruct_worldline w t = (\<sigma>, \<gamma>, \<theta>, \<tau>)" and 
-    "t, \<sigma>, \<gamma>, \<theta> \<turnstile> <Bguarded g ss1 ss2, \<tau>> \<longrightarrow>\<^sub>s \<tau>'" and ci1: "context_invariant t \<sigma> \<gamma> \<theta> \<tau>" and 
+  obtain \<sigma> \<gamma> \<theta> \<tau> \<tau>' where des1: "destruct_worldline w t = (\<sigma>, \<gamma>, \<theta>, \<tau>)" and
+    "t, \<sigma>, \<gamma>, \<theta> \<turnstile> <Bguarded g ss1 ss2, \<tau>> \<longrightarrow>\<^sub>s \<tau>'" and ci1: "context_invariant t \<sigma> \<gamma> \<theta> \<tau>" and
     "w = worldline2 t \<sigma> \<theta> \<tau>" using destruct_worldline_exist worldline2_constructible by blast
   moreover have "\<not> beval t \<sigma> \<gamma> \<theta> g"
     using assms `w = worldline2 t \<sigma> \<theta> \<tau>` ci1  apply transfer' using beval_beval_world_ci by metis
   ultimately have "t, \<sigma>, \<gamma>, \<theta> \<turnstile> <ss2, \<tau>> \<longrightarrow>\<^sub>s \<tau>'"
     by auto
   thus ?thesis
-    by (metis (no_types, lifting) \<open>t , \<sigma> , \<gamma> , \<theta> \<turnstile> <Bguarded g ss1 ss2 , \<tau>> \<longrightarrow>\<^sub>s \<tau>'\<close> case_prod_conv 
+    by (metis (no_types, lifting) \<open>t , \<sigma> , \<gamma> , \<theta> \<turnstile> <Bguarded g ss1 ss2 , \<tau>> \<longrightarrow>\<^sub>s \<tau>'\<close> case_prod_conv
         des1 world_seq_exec_def)
 qed
 
 definition wp :: "'signal seq_stmt \<Rightarrow> nat \<Rightarrow> 'signal assn2 \<Rightarrow> 'signal assn2" where
   "wp ss t Q = (\<lambda>w. \<forall>w'. (w, t, ss \<Rightarrow>\<^sub>s w') \<longrightarrow> Q w')"
 
-lemma wp_bnull: 
+lemma wp_bnull:
   "wp Bnull t Q = Q"
   by (rule ext)(auto simp add: wp_def world_seq_exec_bnull)
 
@@ -1760,20 +1770,20 @@ lemma wp_bcomp:
   "nonneg_delay (Bcomp ss1 ss2) \<Longrightarrow> wp (Bcomp ss1 ss2) t Q = wp ss1 t (wp ss2 t Q)"
   by (rule ext) (auto simp add: wp_def world_seq_exec_comp)
 
-lemma wp_guarded: 
-  "wp (Bguarded g ss1 ss2) t Q = 
+lemma wp_guarded:
+  "wp (Bguarded g ss1 ss2) t Q =
   (\<lambda>w. if beval_world2 w t g then wp ss1 t Q w else wp ss2 t Q w)"
   by (rule ext) (auto simp add: wp_def world_seq_exec_guarded world_seq_exec_guarded_not)
 
-lemma wp_trans: 
-  "wp (Bassign_trans sig exp dly) t Q = 
+lemma wp_trans:
+  "wp (Bassign_trans sig exp dly) t Q =
   (\<lambda>w. Q(w[sig, t + dly :=\<^sub>2 beval_world2 w t exp]))"
   by (rule ext, metis VHDL_Hoare_Complete.wp_def lift_world_trans_worldline_upd2)
 
-lemma wp_inert: 
-  "0 < dly \<Longrightarrow> wp (Bassign_inert sig exp dly) t Q = 
+lemma wp_inert:
+  "0 < dly \<Longrightarrow> wp (Bassign_inert sig exp dly) t Q =
   (\<lambda>w. Q(w[sig, t, dly :=\<^sub>2 beval_world2 w t exp]))"
-  by (rule ext, metis VHDL_Hoare_Complete.wp_def lift_world_inert_worldline_upd2) 
+  by (rule ext, metis VHDL_Hoare_Complete.wp_def lift_world_inert_worldline_upd2)
 
 lemma wp_is_pre: "nonneg_delay ss \<Longrightarrow> \<turnstile>\<^sub>t [wp ss t Q] ss [Q]"
 proof (induction ss arbitrary: Q)
@@ -1803,9 +1813,278 @@ proof (rule strengthen_pre_hoare2)
     using assms by (intro wp_is_pre)
 qed
 
-corollary hoare_sound_complete: 
+corollary hoare_sound_complete:
   assumes "nonneg_delay ss"
   shows "\<turnstile>\<^sub>t [P] ss [Q] \<longleftrightarrow> \<Turnstile>\<^sub>t [P] ss [Q]"
   using hoare_complete soundness_hoare2 assms by auto
+
+subsection \<open>Hoare logic for VHDL's concurrent statement\<close>
+
+definition event_of :: "'signal worldline2  \<Rightarrow> nat \<Rightarrow> 'signal event" where
+  "event_of w t = (fst o snd) (destruct_worldline w t)"
+
+inductive
+  conc_hoare :: "nat \<Rightarrow> 'signal assn2 \<Rightarrow> 'signal conc_stmt \<Rightarrow> 'signal assn2 \<Rightarrow> bool"
+  ("\<turnstile>\<^sub>_ (\<lbrace>(1_)\<rbrace>/ (_)/ \<lbrace>(1_)\<rbrace>)" 50)
+  where
+Single:  "\<turnstile>\<^sub>t [\<lambda>w. P w \<and> \<not> disjnt sl (event_of w t)] ss [Q] \<Longrightarrow> \<forall>w. P w \<and> disjnt sl (event_of w t) \<longrightarrow> Q w
+    \<Longrightarrow> \<turnstile>\<^sub>t \<lbrace>P\<rbrace> process sl : ss \<lbrace>Q\<rbrace>"
+| Parallel:  "\<turnstile>\<^sub>t \<lbrace>P\<rbrace> cs\<^sub>1 \<lbrace>R\<rbrace> \<Longrightarrow> \<turnstile>\<^sub>t \<lbrace>R\<rbrace> cs\<^sub>2 \<lbrace>Q\<rbrace> \<Longrightarrow> conc_stmt_wf (cs\<^sub>1 || cs\<^sub>2) \<Longrightarrow> \<turnstile>\<^sub>t \<lbrace>P\<rbrace> cs\<^sub>1 || cs\<^sub>2 \<lbrace>Q\<rbrace>"
+| Parallel2: "\<turnstile>\<^sub>t \<lbrace>P\<rbrace> cs\<^sub>2 \<lbrace>R\<rbrace> \<Longrightarrow> \<turnstile>\<^sub>t \<lbrace>R\<rbrace> cs\<^sub>1 \<lbrace>Q\<rbrace> \<Longrightarrow> conc_stmt_wf (cs\<^sub>1 || cs\<^sub>2) \<Longrightarrow> \<turnstile>\<^sub>t \<lbrace>P\<rbrace> cs\<^sub>1 || cs\<^sub>2 \<lbrace>Q\<rbrace>"
+
+definition world_conc_exec :: "'signal worldline2 \<Rightarrow> nat \<Rightarrow> 'signal conc_stmt \<Rightarrow> 'signal worldline2"
+  where
+  "world_conc_exec w t c = (let (\<sigma>, \<gamma>, \<theta>, \<tau>) = destruct_worldline w t;
+                                          \<tau>' = b_conc_exec t \<sigma> \<gamma> \<theta> c \<tau>
+                           in worldline2 t \<sigma> \<theta> \<tau>')"
+
+abbreviation world_conc_exec_abb :: "'signal worldline2 \<Rightarrow> nat \<Rightarrow> 'signal conc_stmt \<Rightarrow> 'signal worldline2 \<Rightarrow> bool"
+  ("(_, _ , _) \<Rightarrow>\<^sub>c _")
+  where "world_conc_exec_abb w t s w' \<equiv> (world_conc_exec w t s = w')"
+
+(* Diagram for lifting the concurrent execution to the worldline level
+ *
+ *         w, t                    \<Rightarrow>\<^sub>c          w', t
+ *           \<down>                                  \<up>
+ *   destruct_worldline                      worldline2 t \<sigma> \<theta> \<tau>'
+ *           \<down>                                  \<up>
+ *         t, \<sigma>, \<gamma>, \<theta> \<turnstile> <c, \<tau>>    \<longrightarrow>\<^sub>c          \<tau>'
+ *
+ *)
+
+lemma world_conc_exec_commute:
+  assumes "w, t, (cs1 || cs2) \<Rightarrow>\<^sub>c w1"
+  assumes "w, t, (cs2 || cs1) \<Rightarrow>\<^sub>c w2"
+  assumes "conc_stmt_wf (cs1 || cs2)"
+  shows "w1 = w2"
+proof -
+  obtain \<sigma> \<gamma> \<theta> \<tau> \<tau>' where "destruct_worldline w t = (\<sigma>, \<gamma>, \<theta>, \<tau>)" and
+    "t, \<sigma>, \<gamma>, \<theta> \<turnstile> <cs1 || cs2, \<tau>> \<longrightarrow>\<^sub>c \<tau>'" and "worldline2 t \<sigma> \<theta> \<tau>' = w1"
+    using assms(1) unfolding world_conc_exec_def Let_def by (auto split:prod.splits)
+  hence "t, \<sigma>, \<gamma>, \<theta> \<turnstile> <cs2 || cs1, \<tau>> \<longrightarrow>\<^sub>c \<tau>'"
+    using parallel_comp_commute'[OF assms(3)] by auto
+  thus ?thesis
+    using assms(2) unfolding world_conc_exec_def Let_def
+    using \<open>destruct_worldline w t = (\<sigma>, \<gamma>, \<theta>, \<tau>)\<close> \<open>worldline2 t \<sigma> \<theta> \<tau>' = w1\<close> by auto
+qed
+
+definition
+conc_hoare_valid :: "nat \<Rightarrow> 'signal assn2 \<Rightarrow> 'signal conc_stmt \<Rightarrow> 'signal assn2 \<Rightarrow> bool" ("\<Turnstile>\<^sub>_ \<lbrace>(1_)\<rbrace>/ (_)/ \<lbrace>(1_)\<rbrace>" 50)
+where "\<Turnstile>\<^sub>t \<lbrace>P\<rbrace> c \<lbrace>Q\<rbrace> \<longleftrightarrow>  (\<forall>w w'.  P w \<and> (w, t, c \<Rightarrow>\<^sub>c w') \<longrightarrow> Q w')"
+
+lemma helper_b_conc:
+  assumes "t, \<sigma>, \<gamma>, \<theta>1 \<turnstile> <cs, \<tau>1> \<longrightarrow>\<^sub>c \<tau>1'"
+  assumes "\<And>k s. signal_of2 False \<theta>1 s k = signal_of2 False \<theta>2 s k"
+  assumes "\<And>k s. signal_of2 (\<sigma> s) \<tau>1 s k = signal_of2 (\<sigma> s) \<tau>2 s k"
+  assumes "t, \<sigma>, \<gamma>, \<theta>2 \<turnstile> <cs, \<tau>2> \<longrightarrow>\<^sub>c \<tau>2'"
+  assumes "context_invariant t \<sigma> \<gamma> \<theta>1 \<tau>1" and "context_invariant t \<sigma> \<gamma> \<theta>2 \<tau>2"
+  assumes "nonneg_delay_conc cs"
+  shows "\<And>k s. signal_of2 (\<sigma> s) \<tau>1' s k = signal_of2 (\<sigma> s) \<tau>2' s k"
+  using assms
+proof (induction cs arbitrary: \<tau>1 \<tau>2 \<tau>1' \<tau>2')
+  case (Bpar cs1 cs2)
+  define \<tau>11 where "\<tau>11 = b_conc_exec t \<sigma> \<gamma> \<theta>1 cs1 \<tau>1"
+  define \<tau>12 where "\<tau>12 = b_conc_exec t \<sigma> \<gamma> \<theta>1 cs2 \<tau>1"
+  hence \<tau>1'_def: "\<tau>1' = clean_zip \<tau>1 (\<tau>11, set (signals_from cs1)) (\<tau>12, set (signals_from cs2))"
+    using \<tau>11_def using Bpar by auto
+  define \<tau>21 where "\<tau>21 = b_conc_exec t \<sigma> \<gamma> \<theta>2 cs1 \<tau>2"
+  define \<tau>22 where "\<tau>22 = b_conc_exec t \<sigma> \<gamma> \<theta>2 cs2 \<tau>2"
+  hence \<tau>2'_def: "\<tau>2' = clean_zip \<tau>2 (\<tau>21, set (signals_from cs1)) (\<tau>22, set (signals_from cs2))"
+    using \<tau>21_def using Bpar by auto
+  hence ind1: "\<And>s k. signal_of2 (\<sigma> s) \<tau>11 s k = signal_of2 (\<sigma> s) \<tau>21 s k"
+    using Bpar(1)[OF _ Bpar(4-5) _ Bpar(7-8), of "\<tau>11" "\<tau>21"] Bpar(9) \<tau>11_def \<tau>21_def by auto
+  hence ind2: "\<And>s k. signal_of2 (\<sigma> s) \<tau>12 s k = signal_of2 (\<sigma> s) \<tau>22 s k"
+    using Bpar(2)[OF _ Bpar(4-5) _ Bpar(7-8), of "\<tau>12" "\<tau>22"] Bpar(9) \<tau>12_def \<tau>22_def by auto
+  have "s \<in> set (signals_from cs1) \<or> s \<notin> set (signals_from cs1) \<and> s \<in> set (signals_from cs2) \<or>
+        s \<notin> set (signals_from cs1) \<and> s \<notin> set (signals_from cs2)"
+    by auto
+  moreover
+  { assume "s \<in> set (signals_from cs1)"
+    hence "\<And>n. lookup (to_transaction2 \<tau>1' s) = lookup (to_transaction2 \<tau>11 s)"
+      using \<tau>1'_def apply transfer'
+      unfolding to_trans_raw2_def clean_zip_raw_def Let_def by (auto split:prod.splits)
+    moreover have "\<And>n. lookup (to_transaction2 \<tau>2' s) = lookup (to_transaction2 \<tau>21 s)"
+      using `s \<in> set (signals_from cs1)` \<tau>2'_def apply transfer'
+      unfolding to_trans_raw2_def clean_zip_raw_def Let_def by (auto split:prod.splits)
+    ultimately have  ?case
+      using signal_of2_lookup_sig_same ind1 ind2 by metis }
+  moreover
+  { assume *: "s \<notin> set (signals_from cs1) \<and> s \<in> set (signals_from cs2)"
+    hence "\<And>n. lookup (to_transaction2 \<tau>1' s) = lookup (to_transaction2 \<tau>12 s)"
+      using \<tau>1'_def apply transfer'
+      unfolding to_trans_raw2_def clean_zip_raw_def Let_def by (auto split:prod.splits)
+    moreover have "\<And>n. lookup (to_transaction2 \<tau>2' s) = lookup (to_transaction2 \<tau>22 s)"
+      using * \<tau>2'_def apply transfer'
+      unfolding to_trans_raw2_def clean_zip_raw_def Let_def by (auto split:prod.splits)
+    ultimately have  ?case
+      using signal_of2_lookup_sig_same ind1 ind2 by metis }
+  moreover
+  { assume *: "s \<notin> set (signals_from cs1) \<and> s \<notin> set (signals_from cs2)"
+    hence "\<And>n. lookup (to_transaction2 \<tau>1' s) = lookup (to_transaction2 \<tau>1 s)"
+      using \<tau>1'_def apply transfer'
+      unfolding to_trans_raw2_def clean_zip_raw_def Let_def by (auto split:prod.splits)
+    moreover have "\<And>n. lookup (to_transaction2 \<tau>2' s) = lookup (to_transaction2 \<tau>2 s)"
+      using * \<tau>2'_def apply transfer'
+      unfolding to_trans_raw2_def clean_zip_raw_def Let_def by (auto split:prod.splits)
+    ultimately have  ?case
+      using signal_of2_lookup_sig_same ind1 ind2 Bpar(5) by metis }
+  ultimately show ?case by auto
+next
+  case (Bsingle sl ss)
+  have "disjnt sl \<gamma> \<or> \<not> disjnt sl \<gamma>"
+    by auto
+  moreover
+  { assume "disjnt sl \<gamma>"
+    hence "\<tau>1' = \<tau>1" and "\<tau>2' = \<tau>2"
+      using Bsingle by auto
+    with Bsingle(3) have ?case by auto }
+  moreover
+  { assume "\<not> disjnt sl \<gamma>"
+    hence tau1': "t, \<sigma>, \<gamma>, \<theta>1 \<turnstile> <ss, \<tau>1> \<longrightarrow>\<^sub>s \<tau>1'" and tau2': "t, \<sigma>, \<gamma>, \<theta>2 \<turnstile> <ss, \<tau>2> \<longrightarrow>\<^sub>s \<tau>2'"
+      using Bsingle by auto
+    have "nonneg_delay ss"
+      using Bsingle by auto
+    hence ?case
+      using helper'[OF tau1' Bsingle(2-3) tau2' Bsingle(5-6)] by auto }
+  ultimately show ?case by auto
+qed
+
+lemma parallel_valid:
+  assumes "\<Turnstile>\<^sub>t \<lbrace>P\<rbrace> c1 \<lbrace>R\<rbrace>" and "\<Turnstile>\<^sub>t \<lbrace>R\<rbrace> c2 \<lbrace>Q\<rbrace>" and "conc_stmt_wf (c1 || c2)"
+  assumes "nonneg_delay_conc (c1 || c2)"
+  shows "\<Turnstile>\<^sub>t \<lbrace>P\<rbrace> c1 || c2 \<lbrace>Q\<rbrace>"
+  unfolding conc_hoare_valid_def
+proof rule+
+  fix w w'
+  assume "P w \<and> w, t , c1 || c2 \<Rightarrow>\<^sub>c w'"
+  hence "P w" and "w, t, c1 || c2 \<Rightarrow>\<^sub>c w'"
+    by auto
+  then obtain \<sigma> \<gamma> \<theta> \<tau> \<tau>' where des: "destruct_worldline w t = (\<sigma>, \<gamma>, \<theta>, \<tau>)" and
+    *: "t, \<sigma>, \<gamma>, \<theta> \<turnstile> <c1 || c2, \<tau>> \<longrightarrow>\<^sub>c \<tau>'" and w'_def: "worldline2 t \<sigma> \<theta> \<tau>' = w'" and
+    ci: "context_invariant t \<sigma> \<gamma> \<theta> \<tau>"
+    unfolding world_conc_exec_def Let_def  using destruct_worldline_exist
+    by (metis (mono_tags, lifting) old.prod.case worldline2_constructible)
+  define \<tau>1 where "\<tau>1 = b_conc_exec t \<sigma> \<gamma> \<theta> c1 \<tau>"
+  hence ci1: "context_invariant t \<sigma> \<gamma> \<theta> \<tau>1"
+    using b_conc_exec_preserves_context_invariant[OF ci] assms(4) by auto
+  define \<tau>2 where "\<tau>2 = b_conc_exec t \<sigma> \<gamma> \<theta> c2 \<tau>"
+  hence ci2: "context_invariant t \<sigma> \<gamma> \<theta> \<tau>2"
+    using b_conc_exec_preserves_context_invariant[OF ci] assms(4) by auto
+  have \<tau>'_def: "\<tau>' = b_conc_exec t \<sigma> \<gamma> \<theta> c2 \<tau>1"
+    using b_conc_exec_sequential[OF assms(3)] * unfolding \<tau>1_def by auto
+  define w1 where "w1 = worldline2 t \<sigma> \<theta> \<tau>1"
+  have "w, t, c1 \<Rightarrow>\<^sub>c w1"
+    using des \<tau>1_def unfolding world_conc_exec_def Let_def by (simp add: w1_def)
+  hence "R w1"
+    using assms(1) `P w` unfolding conc_hoare_valid_def by auto
+  obtain theta1 tau1 where des2: "destruct_worldline w1 t = (\<sigma>, \<gamma>, theta1, tau1)" and
+    beh_same: "\<And>k s. signal_of2 False \<theta> s k = signal_of2 False theta1 s k" and
+    trans_same: "\<And>k s. signal_of2 (\<sigma> s) \<tau>1 s k = signal_of2 (\<sigma> s) tau1 s k"
+    using destruct_worldline_exist[of "worldline2 t \<sigma> \<theta> \<tau>1" "t"] unfolding w1_def
+    using destruct_worldline_correctness[OF ci1] by metis
+  have "context_invariant t \<sigma> \<gamma> theta1 tau1"
+    using des2 worldline2_constructible by blast
+  moreover have "nonneg_delay_conc c2"
+    using assms(4) by auto
+  ultimately have "worldline2 t \<sigma> theta1 (b_conc_exec t \<sigma> \<gamma> theta1 c2 tau1) = worldline2 t \<sigma> \<theta> \<tau>'"
+    using beh_same trans_same \<tau>'_def ci1
+  proof (transfer')
+    fix \<sigma> :: "'a state"
+    fix \<theta> theta1 :: "'a transaction"
+    fix \<tau>1 tau1 \<tau>'
+    fix t \<gamma> c2
+    assume bs: "\<And>s k. signal_of2 False \<theta> s k = signal_of2 False theta1 s k"
+    assume ts: "\<And>s k. signal_of2 (\<sigma> s) \<tau>1 s k = signal_of2 (\<sigma> s) tau1 s k"
+    assume \<tau>'_def': "\<tau>' = b_conc_exec t \<sigma> \<gamma> \<theta> c2 \<tau>1"
+    assume ci1': " context_invariant t \<sigma> \<gamma> \<theta> \<tau>1"
+    assume ci2': "context_invariant t \<sigma> \<gamma> theta1 tau1"
+    assume "nonneg_delay_conc c2"
+    hence "\<And>k s. signal_of2 (\<sigma> s) (b_conc_exec t \<sigma> \<gamma> theta1 c2 tau1) s k =
+          signal_of2 (\<sigma> s) (b_conc_exec t \<sigma> \<gamma> \<theta> c2 \<tau>1) s k"
+      using helper_b_conc[OF _ bs ts _ ci1' ci2'] \<tau>'_def' by metis
+    thus "worldline t \<sigma> theta1 (b_conc_exec t \<sigma> \<gamma> theta1 c2 tau1) = worldline t \<sigma> \<theta> \<tau>'"
+      unfolding worldline_def \<tau>'_def' using bs by auto
+  qed
+  hence "w1, t , c2 \<Rightarrow>\<^sub>c w'"
+    using des2 by (simp add: w'_def world_conc_exec_def)
+  with `R w1` show "Q w'"
+    using assms(2) using conc_hoare_valid_def by metis
+qed
+
+lemma soundness_conc_hoare:
+  assumes "\<turnstile>\<^sub>t \<lbrace>P\<rbrace> c \<lbrace>Q\<rbrace>"
+  assumes "conc_stmt_wf c" and "nonneg_delay_conc c"
+  shows "\<Turnstile>\<^sub>t \<lbrace>P\<rbrace> c \<lbrace>Q\<rbrace>"
+  using assms
+proof (induction rule:conc_hoare.induct)
+  case (Single t P sl ss Q)
+  { fix w w'
+    assume as: "P w \<and> (w, t ,  process sl : ss \<Rightarrow>\<^sub>c w')"
+    then obtain \<sigma> \<gamma> \<theta> \<tau> \<tau>' where des: "destruct_worldline w t = (\<sigma>, \<gamma>, \<theta>, \<tau>)" and "P w" and
+      ex: "t, \<sigma>, \<gamma>, \<theta> \<turnstile> <process sl : ss, \<tau>> \<longrightarrow>\<^sub>c \<tau>'" and "worldline2 t \<sigma> \<theta> \<tau>' = w'"
+      unfolding world_seq_exec_def Let_def
+      by (smt case_prod_conv destruct_worldline_exist world_conc_exec_def)
+    have "nonneg_delay ss"
+      using Single by auto
+    have "disjnt sl \<gamma> \<or> \<not> disjnt sl \<gamma>"
+      by auto
+    moreover
+    { assume "disjnt sl \<gamma>"
+      hence "\<tau>' = \<tau>" using ex by auto
+      hence "w' = w"
+        using \<open>destruct_worldline w t = (\<sigma>, \<gamma>, \<theta>, \<tau>)\<close> \<open>worldline2 t \<sigma> \<theta> \<tau>' = w'\<close> worldline2_constructible
+        by blast
+      with Single have "Q w'"
+        unfolding event_of_def  using \<open>P w \<and> w, t , process sl : ss \<Rightarrow>\<^sub>c w'\<close>
+        \<open>destruct_worldline w t = (\<sigma>, \<gamma>, \<theta>, \<tau>)\<close> \<open>disjnt sl \<gamma>\<close>  disjnt_sym by fastforce }
+    moreover
+    { assume "\<not> disjnt sl \<gamma>"
+      hence "\<not> disjnt sl (event_of w t)"
+        unfolding event_of_def using des by auto
+      moreover have "w, t, ss \<Rightarrow>\<^sub>s w'"
+        using as `\<not> disjnt sl \<gamma>`
+      proof -
+        have "t , \<sigma> , \<gamma> , \<theta> \<turnstile> <ss , \<tau>> \<longrightarrow>\<^sub>s \<tau>'"
+          using \<open>\<not> disjnt sl \<gamma>\<close> ex by force
+        then show ?thesis
+          by (simp add: \<open>worldline2 t \<sigma> \<theta> \<tau>' = w'\<close> des world_seq_exec_def)
+      qed
+      ultimately have "Q w'"
+        using soundness_hoare2[OF Single(1) `nonneg_delay ss`] `P w` unfolding seq_hoare_valid2_def
+        by auto }
+    ultimately have "Q w'" by auto }
+  then show ?case
+    unfolding conc_hoare_valid_def by auto
+next
+  case (Parallel t P cs\<^sub>1 R cs\<^sub>2 Q)
+  hence "conc_stmt_wf cs\<^sub>1" and "conc_stmt_wf cs\<^sub>2"
+    by (simp add: conc_stmt_wf_def)+
+  moreover have "nonneg_delay_conc cs\<^sub>1" and "nonneg_delay_conc cs\<^sub>2"
+    using Parallel by auto
+  ultimately have " \<Turnstile>\<^sub>t \<lbrace>P\<rbrace> cs\<^sub>1 \<lbrace>R\<rbrace>" and " \<Turnstile>\<^sub>t \<lbrace>R\<rbrace> cs\<^sub>2 \<lbrace>Q\<rbrace>"
+    using Parallel by auto
+  then show ?case
+    using parallel_valid Parallel by blast
+next
+  case (Parallel2 t P cs\<^sub>2 R cs\<^sub>1 Q)
+  hence "conc_stmt_wf cs\<^sub>1" and "conc_stmt_wf cs\<^sub>2"
+    by (simp add: conc_stmt_wf_def)+
+  moreover have "nonneg_delay_conc cs\<^sub>1" and "nonneg_delay_conc cs\<^sub>2"
+    using Parallel2 by auto
+  ultimately have cs2: " \<Turnstile>\<^sub>t \<lbrace>P\<rbrace> cs\<^sub>2 \<lbrace>R\<rbrace>" and cs1: " \<Turnstile>\<^sub>t \<lbrace>R\<rbrace> cs\<^sub>1 \<lbrace>Q\<rbrace>"
+    using Parallel2 by auto
+  have "conc_stmt_wf (cs\<^sub>2 || cs\<^sub>1)"
+    using Parallel2(3) unfolding conc_stmt_wf_def by auto
+  moreover have " nonneg_delay_conc (cs\<^sub>2 || cs\<^sub>1) "
+    using Parallel2(7) by auto
+  ultimately have "\<Turnstile>\<^sub>t \<lbrace>P\<rbrace> cs\<^sub>2 || cs\<^sub>1 \<lbrace>Q\<rbrace>"
+    using parallel_valid[OF cs2 cs1]   by auto
+  thus ?case
+    using world_conc_exec_commute[OF _ _ Parallel2(3)]  by (metis conc_hoare_valid_def)
+qed
+
+
+
+
 
 end
